Optimized proofs with derivatives.

HybridVerifVecs/funcsets/cat2funcset.thy
@@ -12,18 +12,18 @@ section \<open>Verification of regular programs\<close>
 
 text \<open>First we add lemmas for computation of weakest liberal preconditions (wlps).\<close>
 
-lemma ffb_eta[simp]:"fb\<^sub>\<F> \<eta> X = X"
+lemma ffb_eta[simp]: "fb\<^sub>\<F> \<eta> X = X"
   unfolding ffb_def by(simp add: kop_def klift_def map_dual_def)
 
-lemma ffb_eq:"fb\<^sub>\<F> F X = {s. \<forall>y. y \<in> F s \<longrightarrow> y \<in> X}"
+lemma ffb_eq: "fb\<^sub>\<F> F X = {s. \<forall>y. y \<in> F s \<longrightarrow> y \<in> X}"
   unfolding ffb_def apply(simp add: kop_def klift_def map_dual_def)
   unfolding dual_set_def f2r_def r2f_def by auto
 
-lemma ffb_eq_univD:"fb\<^sub>\<F> F P = UNIV \<Longrightarrow> (\<forall>y. y \<in> (F x) \<longrightarrow> y \<in> P)"
+lemma ffb_eq_univD: "fb\<^sub>\<F> F P = UNIV \<Longrightarrow> (\<forall>y. y \<in> (F x) \<longrightarrow> y \<in> P)"
 proof
   fix y assume "fb\<^sub>\<F> F P = UNIV"
   hence "UNIV = {s. \<forall>y. y \<in> (F s) \<longrightarrow> y \<in> P}" 
-    by(subst ffb_eq[THEN sym], simp)
+    by(subst ffb_eq[symmetric], simp)
   hence "\<And>x. {x} = {s. s = x \<and> (\<forall>y. y \<in> (F s) \<longrightarrow> y \<in> P)}" 
     by auto
   then show "s2p (F x) y \<longrightarrow> y \<in> P" 
@@ -32,18 +32,18 @@ qed
 
 text \<open>Next, we introduce assignments and their wlps.\<close>
 
-abbreviation vec_upd :: "('a^'b) \<Rightarrow> 'b \<Rightarrow> 'a \<Rightarrow> 'a^'b" ("_(2[_ :== _])" [70, 65] 61) 
-  where "x[i :== a] \<equiv> (\<chi> j. (if j = i then a else (x $ j)))"
+abbreviation vec_upd :: "('a^'b) \<Rightarrow> 'b \<Rightarrow> 'a \<Rightarrow> 'a^'b"
+  where "vec_upd x i a \<equiv> vec_lambda ((vec_nth x)(i := a))"
 
-abbreviation assign :: "'b \<Rightarrow> ('a^'b \<Rightarrow> 'a) \<Rightarrow> ('a^'b) \<Rightarrow> ('a^'b) set" ("(2[_ ::== _])" [70, 65] 61) 
-  where "[x ::== expr]\<equiv> (\<lambda>s. {s[x :== expr s]})" 
+abbreviation assign :: "'b \<Rightarrow> ('a^'b \<Rightarrow> 'a) \<Rightarrow> ('a^'b) \<Rightarrow> ('a^'b) set" ("(2_ ::= _)" [70, 65] 61) 
+  where "(x ::= e) \<equiv> (\<lambda>s. {vec_upd s x (e s)})" 
 
-lemma ffb_assign[simp]: "fb\<^sub>\<F> ([x ::== expr]) Q = {s. (s[x :== expr s]) \<in> Q}"
-  by(subst ffb_eq, simp)
+lemma ffb_assign[simp]: "fb\<^sub>\<F> (x ::= e) Q = {s. (vec_upd s x (e s)) \<in> Q}"
+  by(subst ffb_eq) simp
 
 text \<open>The wlp of a (kleisli) composition is just the composition of the wlps.\<close>
 
-lemma ffb_kcomp:"fb\<^sub>\<F> (G \<circ>\<^sub>K F) P = fb\<^sub>\<F> G (fb\<^sub>\<F> F P)"
+lemma ffb_kcomp: "fb\<^sub>\<F> (G \<circ>\<^sub>K F) P = fb\<^sub>\<F> G (fb\<^sub>\<F> F P)"
   unfolding ffb_def apply(simp add: kop_def klift_def map_dual_def)
   unfolding dual_set_def f2r_def r2f_def by(auto simp: kcomp_def)
 
@@ -71,25 +71,25 @@ lemma ffb_if_then_elseD:
 
 text \<open>The final wlp we add is that of the finite iteration.\<close>
 
-lemma kstar_inv:"I \<le> {s. \<forall>y. y \<in> F s \<longrightarrow> y \<in> I} \<Longrightarrow> I \<le> {s. \<forall>y. y \<in> (kpower F n s) \<longrightarrow> y \<in> I}"
+lemma kstar_inv: "I \<le> {s. \<forall>y. y \<in> F s \<longrightarrow> y \<in> I} \<Longrightarrow> I \<le> {s. \<forall>y. y \<in> (kpower F n s) \<longrightarrow> y \<in> I}"
   apply(induct n, simp)
   by(auto simp: kcomp_prop) 
 
-lemma ffb_star_induct_self:"I \<le> fb\<^sub>\<F> F I \<Longrightarrow> I \<subseteq> fb\<^sub>\<F> (kstar F) I"
+lemma ffb_star_induct_self: "I \<le> fb\<^sub>\<F> F I \<Longrightarrow> I \<subseteq> fb\<^sub>\<F> (kstar F) I"
   apply(subst ffb_eq, subst (asm) ffb_eq)
   unfolding kstar_def apply clarsimp
   using kstar_inv by blast
 
 lemma ffb_starI:
-assumes "P \<le> I" and "I \<le> fb\<^sub>\<F> F I" and "I \<le> Q"
-shows "P \<le> fb\<^sub>\<F> (kstar F) Q"
+  assumes "P \<le> I" and "I \<le> fb\<^sub>\<F> F I" and "I \<le> Q"
+  shows "P \<le> fb\<^sub>\<F> (kstar F) Q"
 proof-
-  from assms(2) have "I \<subseteq> fb\<^sub>\<F> (kstar F) I"
-    using ffb_star_induct_self by blast
-  then have "P \<le> fb\<^sub>\<F> (kstar F) I"
+  have "I \<subseteq> fb\<^sub>\<F> (kstar F) I"
+    using assms(2) ffb_star_induct_self by blast
+  hence "P \<le> fb\<^sub>\<F> (kstar F) I"
     using assms(1) by auto
-  from this and assms(3) show ?thesis
-    by(subst ffb_eq, subst (asm) ffb_eq, auto)
+  thus ?thesis
+    using assms(3) by(subst ffb_eq, subst (asm) ffb_eq, auto)
 qed
 
 
@@ -113,23 +113,13 @@ lemma ivp_solsD:
     and "x t\<^sub>0 = s" and "t\<^sub>0 \<in> T"
   using assms unfolding ivp_sols_def by auto
 
-text\<open>We use closed segments instead of closed intervals for the following definition due to the 
-following property.\<close>
-
-lemma "(t::real) \<in> {0--t}"
-  by (rule ends_in_segment(2))
-
-lemma "(t::real) \<in> {0..t}"
-  apply auto
-  oops
-
-definition "g_orbital f T t\<^sub>0 G s = \<Union> {{x t|t. t \<in> T \<and> G \<rhd> x {t\<^sub>0--t} }|x. x \<in> ivp_sols f T t\<^sub>0 s}"
+definition "g_orbital f T t\<^sub>0 G s = \<Union> {{x t|t. t \<in> T \<and> G \<rhd> x {t\<^sub>0..t} }|x. x \<in> ivp_sols f T t\<^sub>0 s}"
 
 lemma g_orbital_eq: "g_orbital f T t\<^sub>0 G s =
-  {x t |t x. t \<in> T \<and> (D x = (f \<circ> x) on T) \<and> x t\<^sub>0 = s \<and> t\<^sub>0 \<in> T \<and> G \<rhd> x {t\<^sub>0--t}}"
+  {x t |t x. t \<in> T \<and> (D x = (f \<circ> x) on T) \<and> x t\<^sub>0 = s \<and> t\<^sub>0 \<in> T \<and> G \<rhd> x {t\<^sub>0..t}}"
   unfolding g_orbital_def ivp_sols_def by auto
 
-lemma "g_orbital f T t\<^sub>0 G s = (\<Union> x \<in> ivp_sols f T t\<^sub>0 s. {x t|t. t \<in> T \<and> G \<rhd> x {t\<^sub>0--t}})"
+lemma "g_orbital f T t\<^sub>0 G s = (\<Union> x \<in> ivp_sols f T t\<^sub>0 s. {x t|t. t \<in> T \<and> G \<rhd> x {t\<^sub>0..t}})"
   unfolding g_orbital_def ivp_sols_def by auto
 
 abbreviation g_evol ::"(('a::banach)\<Rightarrow>'a) \<Rightarrow> real set \<Rightarrow> 'a pred \<Rightarrow> 'a \<Rightarrow> 'a set" ("(1[x\<acute>=_]_ & _)") 
@@ -139,7 +129,7 @@ lemmas g_evol_def = g_orbital_eq[where t\<^sub>0=0]
 
 lemma g_evolI:
   assumes "D x = (f \<circ> x) on T" "x 0 = s"
-    and "0 \<in> T" "t \<in> T" and "G \<rhd> x {0--t}"
+    and "0 \<in> T" "t \<in> T" and "G \<rhd> x {0..t}"
   shows "x t \<in> ([x\<acute>=f]T & G) s"
   using assms unfolding g_orbital_def ivp_sols_def by blast
 
@@ -147,7 +137,7 @@ lemma g_evolD:
   assumes "s' \<in> ([x\<acute>=f]T & G) s"
   obtains x and t where "x \<in> ivp_sols f T 0 s" 
   and "D x = (f \<circ> x) on T" "x 0 = s"
-  and "x t = s'" and "0 \<in> T" "t \<in> T" and "G \<rhd> x {0--t}"
+  and "x t = s'" and "0 \<in> T" "t \<in> T" and "G \<rhd> x {0..t}"
   using assms unfolding g_orbital_def ivp_sols_def by blast
 
 context local_flow
@@ -163,24 +153,26 @@ lemma orbit_eq[simp]: "orbit s = {\<phi> t s| t. t \<in> T}"
   by(auto intro: usolves_ivp intro!: ivp simp: init_time)
 
 lemma g_evol_collapses: 
-  shows "([x\<acute>=f]T & G) s = {\<phi> t s| t. t \<in> T \<and> G \<rhd> (\<lambda>r. \<phi> r s) {0--t}}" (is "_ = ?gorbit")
+  shows "([x\<acute>=f]T & G) s = {\<phi> t s| t. t \<in> T \<and> G \<rhd> (\<lambda>r. \<phi> r s) {0..t}}" (is "_ = ?gorbit")
 proof(rule subset_antisym, simp_all only: subset_eq)
   {fix s' assume "s' \<in> ([x\<acute>=f]T & G) s"
-    then obtain x and t where x_ivp:"D x = (f \<circ> x) on T" 
-      "x 0 = s" and "x t = s'" and "t \<in> T" and guard:"G \<rhd> x {0--t}"
-      unfolding g_orbital_eq by blast
-    hence obs:"\<forall>\<tau>\<in>{0--t}. x \<tau> = \<phi> \<tau> s"
-      using usolves_ivp[of x s] closed_segment_subset_domainI init_time comp_def
-      by (metis (mono_tags, lifting) has_vderiv_eq)
-    hence "G \<rhd> (\<lambda>r. \<phi> r s) {0--t}"
+    then obtain x and t where x_ivp:"D x = (\<lambda>t. f (x t)) on T" 
+      "x 0 = s" and "x t = s'" and "t \<in> T" and guard:"G \<rhd> x {0..t}"
+      unfolding g_orbital_eq by auto
+    hence obs:"\<forall>\<tau>\<in>{0..t}. x \<tau> = \<phi> \<tau> s"
+      using usolves_ivp[OF x_ivp] init_time
+      by (meson atLeastAtMost_iff interval_time mem_is_interval_1_I)
+    hence "G \<rhd> (\<lambda>r. \<phi> r s) {0..t}"
       using guard by simp
-    hence "s' \<in> ?gorbit"
-      using \<open>x t = s'\<close> \<open>t \<in> T\<close> obs by blast}
+    also have "\<phi> t s = x t"
+      using usolves_ivp[OF x_ivp \<open>t \<in> T\<close>] by simp
+    ultimately have "s' \<in> ?gorbit"
+      using \<open>x t = s'\<close> \<open>t \<in> T\<close> by auto}
   thus "\<forall>s'\<in>([x\<acute>=f]T & G) s. s' \<in> ?gorbit"
     by blast
 next
   {fix s' assume "s' \<in> ?gorbit"
-    then obtain t where "G \<rhd> (\<lambda>r. \<phi> r s) {0--t}" and "t \<in> T" and "\<phi> t s = s'"
+    then obtain t where "G \<rhd> (\<lambda>r. \<phi> r s) {0..t}" and "t \<in> T" and "\<phi> t s = s'"
       by blast
     hence "s' \<in> ([x\<acute>=f]T & G) s"
       by(auto intro: g_evolI simp: ivp init_time)}
@@ -191,13 +183,15 @@ qed
 lemma ffb_orbit: "fb\<^sub>\<F> (orbit) Q = {s. \<forall> t \<in> T. \<phi> t s \<in> Q}"
   unfolding orbit_eq ffb_eq by auto
 
-lemma ffb_g_orbit: "fb\<^sub>\<F> ([x\<acute>=f]T & G) Q = {s. \<forall>t\<in>T. (G \<rhd> (\<lambda>r. \<phi> r s) {0--t}) \<longrightarrow> (\<phi> t s) \<in> Q}"
+lemma ffb_g_orbit: "fb\<^sub>\<F> ([x\<acute>=f]T & G) Q = {s. \<forall>t\<in>T. (G \<rhd> (\<lambda>r. \<phi> r s) {0..t}) \<longrightarrow> (\<phi> t s) \<in> Q}"
   unfolding g_evol_collapses ffb_eq by auto 
 
 end
 
-lemma (in global_flow) ivp_sols_collapse[simp]: "ivp_sols f UNIV 0 s = {(\<lambda>t. \<phi> t s)}"
-  by(auto intro: usolves_ivp simp: ivp_sols_def ivp)
+lemma (in local_flow) ivp_sols_collapse: "ivp_sols f T 0 s = {(\<lambda>t. \<phi> t s)}"
+  apply(auto simp: ivp_sols_def ivp init_time fun_eq_iff)
+  apply(rule unique_solution, simp_all add: ivp)
+  oops
 
 text\<open> The previous lemma allows us to compute wlps for known systems of ODEs. We can also implement
 a version of it as an inference rule. A simple computation of a wlp is shown immmediately after.\<close>
@@ -206,13 +200,12 @@ lemma dSolution:
   assumes "local_flow f T L \<phi>"
     and "\<forall>s. s \<in> P \<longrightarrow> (\<forall> t \<in> T. (G \<rhd> (\<lambda>r. \<phi> r s) {0..t}) \<longrightarrow> (\<phi> t s) \<in> Q)"
   shows "P \<le> fb\<^sub>\<F> ([x\<acute>=f]T & G) Q"
-  using assms apply(subst local_flow.ffb_g_orbit)
-  by (auto simp: Starlike.closed_segment_eq_real_ivl)
+  using assms by(subst local_flow.ffb_g_orbit) auto
 
 lemma ffb_line: "0 \<le> t \<Longrightarrow> fb\<^sub>\<F> ([x\<acute>=\<lambda>t. c]{0..t} & G) Q = 
     {x. \<forall> \<tau> \<in> {0..t}. (G \<rhd> (\<lambda>r. x + r *\<^sub>R c) {0..\<tau>}) \<longrightarrow> (x + \<tau> *\<^sub>R c) \<in> Q}"
   apply(subst local_flow.ffb_g_orbit[of "\<lambda> t. c" _ "1/(t + 1)" "(\<lambda> t x. x + t *\<^sub>R c)"])
-  by(auto simp: line_is_local_flow closed_segment_eq_real_ivl)
+  by(auto simp: line_is_local_flow)
 
 subsection\<open> Verification with differential invariants \<close>
 
@@ -223,23 +216,22 @@ Then we prove the inference rules which are used in our verification proofs.\<cl
 
 subsubsection\<open> Differential Weakening \<close>
         
-lemma DW:
-  shows "fb\<^sub>\<F> ([x\<acute>=f]T & G) Q = fb\<^sub>\<F> ([x\<acute>=f]T & G) {s. G s \<longrightarrow> s \<in> Q}"
+lemma DW: "fb\<^sub>\<F> ([x\<acute>=f]{0..t} & G) Q = fb\<^sub>\<F> ([x\<acute>=f]{0..t} & G) {s. G s \<longrightarrow> s \<in> Q}"
   by(auto intro: g_evolD simp: ffb_eq)
   
 lemma dWeakening: 
-assumes "{s. G s} \<le> Q"
-shows "P \<le> fb\<^sub>\<F> ([x\<acute>=f]T & G) Q"
+  assumes "{s. G s} \<le> Q"
+  shows "P \<le> fb\<^sub>\<F> ([x\<acute>=f]{0..t} & G) Q"
   using assms by(auto intro: g_evolD simp: le_fun_def g_evol_def ffb_eq)
 
 subsubsection\<open> Differential Cut \<close>
 
 lemma ffb_g_orbit_eq_univD:
   assumes "fb\<^sub>\<F> ([x\<acute>=f]T & G) {s. C s} = UNIV" 
-    and "\<forall> r\<in>{0--t}. x r \<in> ([x\<acute>=f]T & G) s"
-  shows "\<forall>r\<in>{0--t}. C (x r)"
+    and "\<forall> r\<in>{0..t}. x r \<in> ([x\<acute>=f]T & G) s"
+  shows "\<forall>r\<in>{0..t}. C (x r)"
 proof
-  fix r assume "r \<in> {0--t}"
+  fix r assume "r \<in> {0..t}"
   then have "x r \<in> ([x\<acute>=f]T & G) s" 
     using assms(2) by blast
   also have "\<forall>y. y \<in> ([x\<acute>=f]T & G) s \<longrightarrow> C y" 
@@ -254,15 +246,15 @@ proof(rule_tac f="\<lambda> x. fb\<^sub>\<F> x Q" in HOL.arg_cong, rule ext, rul
   fix s 
   {fix s' assume "s' \<in> ([x\<acute>=f]T & G) s"
     then obtain t::real and x where x_ivp: "D x = (f \<circ> x) on T" "x 0 = s"
-      and guard_x:"G \<rhd> x {0--t}" and "s' = x t" and "0 \<in> T" "t \<in> T"
+      and guard_x:"G \<rhd> x {0..t}" and "s' = x t" and "0 \<in> T" "t \<in> T"
       using g_evolD[of s' "f" T G s] by (metis (full_types))
-    from guard_x have "\<forall>r\<in>{0--t}.\<forall> \<tau>\<in>{0--r}. G (x \<tau>)"
-      by (metis contra_subsetD ends_in_segment(1) subset_segment(1))
-    also have "\<forall>\<tau>\<in>{0--t}. \<tau> \<in> T"
-      using interval.closed_segment_subset_domain[OF assms(1) \<open>0 \<in> T\<close> \<open>t \<in> T\<close>] by blast
-    ultimately have "\<forall>\<tau>\<in>{0--t}. x \<tau> \<in> ([x\<acute>=f]T & G) s"
+    from guard_x have "\<forall>r\<in>{0..t}.\<forall> \<tau>\<in>{0..r}. G (x \<tau>)"
+      by auto
+    also have "\<forall>\<tau>\<in>{0..t}. \<tau> \<in> T"
+      by (meson \<open>0 \<in> T\<close> \<open>t \<in> T\<close> assms(1) atLeastAtMost_iff interval.interval mem_is_interval_1_I)
+    ultimately have "\<forall>\<tau>\<in>{0..t}. x \<tau> \<in> ([x\<acute>=f]T & G) s"
       using g_evolI[OF x_ivp \<open>0 \<in> T\<close>] by blast
-    hence "C \<rhd> x {0--t}" 
+    hence "C \<rhd> x {0..t}" 
       using ffb_g_orbit_eq_univD assms(2) by blast
     hence "s' \<in> ([x\<acute>=f]T & (\<lambda>s. G s \<and> C s)) s"
       using g_evolI[OF x_ivp \<open>0 \<in> T\<close> \<open>t \<in> T\<close>] guard_x \<open>s' = x t\<close> by fastforce}
@@ -278,17 +270,17 @@ lemma dCut:
   shows "P \<le> fb\<^sub>\<F> ([x\<acute>=f]{0..t} & G) Q"
 proof(subst ffb_eq, subst g_evol_def, clarsimp)
   fix \<tau>::real and x::"real \<Rightarrow> 'a" assume "(x 0) \<in> P" and "0 \<le> \<tau>" and "\<tau> \<le> t"
-    and x_solves:"D x = (\<lambda>t. f (x t)) on {0..t}" and guard_x:"(\<forall> r \<in> {0--\<tau>}. G (x r))"
-  hence "\<forall>r\<in>{0--\<tau>}.\<forall>\<tau>\<in>{0--r}. G (x \<tau>)"
-    using closed_segment_closed_segment_subset by blast
-  hence "\<forall>r\<in>{0--\<tau>}. x r \<in> ([x\<acute>=f]{0..t} & G) (x 0)"
-    using g_evolI x_solves \<open>0 \<le> \<tau>\<close> \<open>\<tau> \<le> t\<close> closed_segment_eq_real_ivl by fastforce 
-  hence "\<forall>r\<in>{0--\<tau>}. C (x r)" 
+    and x_solves:"D x = (\<lambda>t. f (x t)) on {0..t}" and guard_x:"(\<forall> r \<in> {0..\<tau>}. G (x r))"
+  hence "\<forall>r\<in>{0..\<tau>}.\<forall>\<tau>\<in>{0..r}. G (x \<tau>)"
+    by auto
+  hence "\<forall>r\<in>{0..\<tau>}. x r \<in> ([x\<acute>=f]{0..t} & G) (x 0)"
+    using g_evolI x_solves \<open>0 \<le> \<tau>\<close> \<open>\<tau> \<le> t\<close> by fastforce 
+  hence "\<forall>r\<in>{0..\<tau>}. C (x r)" 
     using ffb_C \<open>(x 0) \<in> P\<close> by(subst (asm) ffb_eq, auto)
   hence "x \<tau> \<in> ([x\<acute>=f]{0..t} & (\<lambda> s. G s \<and> C s)) (x 0)"
     using g_evolI x_solves guard_x \<open>0 \<le> \<tau>\<close> \<open>\<tau> \<le> t\<close> by fastforce
   from this \<open>(x 0) \<in> P\<close> and ffb_Q show "(x \<tau>) \<in> Q"
-    by(subst (asm) ffb_eq, auto simp: closed_segment_eq_real_ivl)
+    by(subst (asm) ffb_eq) auto
 qed
 
 subsubsection\<open> Differential Invariant \<close>
@@ -367,61 +359,61 @@ assumes "I is_diff_invariant_of f along {0..t}"
 
 text\<open> Finally, we obtain some conditions to prove specific instances of differential invariants. \<close>
 
-named_theorems ode_invariant_rules "compilation of rules for differential invariants."
+named_theorems diff_invariant_rules "compilation of rules for differential invariants."
 
-lemma [ode_invariant_rules]:
-fixes \<theta>::"'a::banach \<Rightarrow> real"
-assumes "\<forall> x. (D x = (\<lambda>\<tau>. f (x \<tau>)) on {0..t}) \<longrightarrow> (\<forall> \<tau> \<in> {0..t}. \<forall> r \<in> {0--\<tau>}. 
-  ((\<lambda>\<tau>. \<theta> (x \<tau>) - \<nu> (x \<tau>) ) has_derivative (\<lambda>\<tau>.  \<tau> *\<^sub>R 0)) (at r within {0--\<tau>}))"
-shows "(\<lambda>s. \<theta> s = \<nu> s) is_diff_invariant_of f along {0..t}"
+lemma [diff_invariant_rules]:
+  fixes \<theta>::"'a::banach \<Rightarrow> real"
+  assumes "\<forall>x. (D x = (\<lambda>\<tau>. f (x \<tau>)) on {0..t}) \<longrightarrow> 
+  (\<forall>\<tau>\<in>{0..t}. (D (\<lambda>\<tau>. \<theta> (x \<tau>) - \<nu> (x \<tau>)) = ((*\<^sub>R) 0) on {0..\<tau>}))"
+  shows "(\<lambda>s. \<theta> s = \<nu> s) is_diff_invariant_of f along {0..t}"
 proof(simp add: diff_invariant_def ivp_sols_def, clarsimp)
   fix x \<tau> assume tHyp:"0 \<le> \<tau>" "\<tau> \<le> t" 
     and x_ivp:"D x = (\<lambda>\<tau>. f (x \<tau>)) on {0..t}" "\<theta> (x 0) = \<nu> (x 0)" 
-  hence "\<forall> r \<in> {0--\<tau>}. D (\<lambda>\<tau>. \<theta> (x \<tau>) - \<nu> (x \<tau>)) \<mapsto> (\<lambda>\<tau>. \<tau> *\<^sub>R 0) at r within {0--\<tau>}" 
-    using assms by auto
-  hence "\<exists>r\<in>{0--\<tau>}. (\<theta> (x \<tau>) - \<nu> (x \<tau>)) - (\<theta> (x 0) - \<nu> (x 0)) = (\<lambda>\<tau>. \<tau> *\<^sub>R 0) (\<tau> - 0)" 
-    by(rule_tac closed_segment_mvt, auto simp: tHyp) 
+  hence "\<forall> t \<in> {0..\<tau>}. D (\<lambda>\<tau>. \<theta> (x \<tau>) - \<nu> (x \<tau>)) \<mapsto> (\<lambda>\<tau>. \<tau> *\<^sub>R 0) at t within {0..\<tau>}" 
+    using assms by (auto simp: has_vderiv_on_def has_vector_derivative_def)
+  hence "\<exists>t\<in>{0..\<tau>}. \<theta> (x \<tau>) - \<nu> (x \<tau>) - (\<theta> (x 0) - \<nu> (x 0)) = (\<tau> - 0) \<cdot> 0" 
+    by(rule_tac mvt_very_simple) (auto simp: tHyp)
   thus "\<theta> (x \<tau>) = \<nu> (x \<tau>)" by (simp add: x_ivp(2))
 qed
 
-lemma [ode_invariant_rules]:
-fixes \<theta>::"'a::banach \<Rightarrow> real"
-assumes "\<forall> x. (D x = (\<lambda>\<tau>. f (x \<tau>)) on {0..t}) \<longrightarrow> (\<forall> \<tau> \<in> {0..t}. \<forall> r \<in> {0--\<tau>}. \<theta>' (x r) \<ge> \<nu>' (x r)
-\<and> (D (\<lambda>\<tau>. \<theta> (x \<tau>) - \<nu> (x \<tau>)) \<mapsto> (\<lambda>\<tau>. \<tau> *\<^sub>R (\<theta>' (x r) - \<nu>' (x r))) at r within {0--\<tau>}))"
-shows "(\<lambda>s. \<nu> s \<le> \<theta> s) is_diff_invariant_of f along {0..t}"
+lemma [diff_invariant_rules]:
+  fixes \<theta>::"'a::banach \<Rightarrow> real"
+  assumes "\<forall> x. (D x = (\<lambda>\<tau>. f (x \<tau>)) on {0..t}) \<longrightarrow> (\<forall>\<tau>\<in>{0..t}. \<theta>' (x \<tau>) \<ge> \<nu>' (x \<tau>) \<and> 
+  (D (\<lambda>\<tau>. \<theta> (x \<tau>) - \<nu> (x \<tau>)) = (\<lambda>r. \<theta>' (x r) - \<nu>' (x r)) on {0..\<tau>}))"
+  shows "(\<lambda>s. \<nu> s \<le> \<theta> s) is_diff_invariant_of f along {0..t}"
 proof(simp add: diff_invariant_def ivp_sols_def, clarsimp)
   fix x \<tau> assume tHyp:"0 \<le> \<tau>" "\<tau> \<le> t" 
     and x_ivp:"D x = (\<lambda>\<tau>. f (x \<tau>)) on {0..t}" "\<nu> (x 0) \<le> \<theta> (x 0)"
-  hence primed:"\<forall> r \<in> {0--\<tau>}. (D (\<lambda>\<tau>. \<theta> (x \<tau>) - \<nu> (x \<tau>)) \<mapsto> (\<lambda>\<tau>. \<tau> *\<^sub>R (\<theta>' (x r) - \<nu>' (x r))) 
-  at r within {0--\<tau>}) \<and> \<nu>' (x r) \<le> \<theta>' (x r)" 
-    using assms by auto
-  hence "\<exists>r\<in>{0--\<tau>}. (\<theta> (x \<tau>) - \<nu> (x \<tau>)) - (\<theta> (x 0) - \<nu> (x 0)) = 
+  hence primed:"\<forall> r \<in> {0..\<tau>}. (D (\<lambda>\<tau>. \<theta> (x \<tau>) - \<nu> (x \<tau>)) \<mapsto> (\<lambda>\<tau>. \<tau> *\<^sub>R (\<theta>' (x r) - \<nu>' (x r))) 
+  at r within {0..\<tau>}) \<and> \<nu>' (x r) \<le> \<theta>' (x r)" 
+    using assms by (auto simp: has_vderiv_on_def has_vector_derivative_def)
+  hence "\<exists>r\<in>{0..\<tau>}. (\<theta> (x \<tau>) - \<nu> (x \<tau>)) - (\<theta> (x 0) - \<nu> (x 0)) = 
   (\<lambda>\<tau>. \<tau> *\<^sub>R (\<theta>' (x r) -  \<nu>' (x r))) (\<tau> - 0)" 
-    by(rule_tac closed_segment_mvt, auto simp: \<open>0 \<le> \<tau>\<close>)
-  then obtain r where "r \<in> {0--\<tau>}" 
+    by(rule_tac mvt_very_simple) (auto simp: tHyp)
+  then obtain r where "r \<in> {0..\<tau>}" 
     and "\<theta> (x \<tau>) - \<nu> (x \<tau>) = (\<tau> - 0) *\<^sub>R (\<theta>' (x r) -  \<nu>' (x r)) + (\<theta> (x 0) - \<nu> (x 0))" 
     by force 
   also have "... \<ge> 0" 
-    using tHyp(1) x_ivp(2) primed by (simp add: calculation(1))  
+    using tHyp(1) x_ivp(2) primed calculation(1) by auto 
   ultimately show "\<nu> (x \<tau>) \<le> \<theta> (x \<tau>)" 
     by simp
 qed
 
-lemma [ode_invariant_rules]:
+lemma [diff_invariant_rules]:
 fixes \<theta>::"'a::banach \<Rightarrow> real"
-assumes "\<forall> x. (D x = (\<lambda>\<tau>. f (x \<tau>)) on {0..t}) \<longrightarrow> (\<forall> \<tau> \<in> {0..t}. \<forall> r \<in> {0--\<tau>}. \<theta>' (x r) \<ge> \<nu>' (x r)
-\<and> (D (\<lambda>\<tau>. \<theta> (x \<tau>) - \<nu> (x \<tau>)) \<mapsto> (\<lambda>\<tau>. \<tau> *\<^sub>R (\<theta>' (x r) - \<nu>' (x r))) at r within {0--\<tau>}))"
+assumes "\<forall> x. (D x = (\<lambda>\<tau>. f (x \<tau>)) on {0..t}) \<longrightarrow> (\<forall>\<tau>\<in>{0..t}. \<theta>' (x \<tau>) \<ge> \<nu>' (x \<tau>) \<and> 
+  (D (\<lambda>\<tau>. \<theta> (x \<tau>) - \<nu> (x \<tau>)) = (\<lambda>r. \<theta>' (x r) - \<nu>' (x r)) on {0..\<tau>}))"
 shows "(\<lambda>s. \<nu> s < \<theta> s) is_diff_invariant_of f along {0..t}"
 proof(simp add: diff_invariant_def ivp_sols_def, clarsimp)
   fix x \<tau> assume tHyp:"0 \<le> \<tau>" "\<tau> \<le> t"
     and x_ivp:"D x = (\<lambda>\<tau>. f (x \<tau>)) on {0..t}" "\<nu> (x 0) < \<theta> (x 0)"
-  hence primed:"\<forall> r \<in> {0--\<tau>}. ((\<lambda>\<tau>. \<theta> (x \<tau>) - \<nu> (x \<tau>)) has_derivative 
-(\<lambda>\<tau>. \<tau> *\<^sub>R  (\<theta>' (x r) -  \<nu>' (x r)))) (at r within {0--\<tau>}) \<and> \<theta>' (x r) \<ge> \<nu>' (x r)" 
-    using assms by auto
-  hence "\<exists>r\<in>{0--\<tau>}. (\<theta> (x \<tau>) - \<nu> (x \<tau>)) - (\<theta> (x 0) - \<nu> (x 0)) = 
+  hence primed:"\<forall> r \<in> {0..\<tau>}. ((\<lambda>\<tau>. \<theta> (x \<tau>) - \<nu> (x \<tau>)) has_derivative 
+(\<lambda>\<tau>. \<tau> *\<^sub>R  (\<theta>' (x r) -  \<nu>' (x r)))) (at r within {0..\<tau>}) \<and> \<theta>' (x r) \<ge> \<nu>' (x r)" 
+    using assms by (auto simp: has_vderiv_on_def has_vector_derivative_def)
+  hence "\<exists>r\<in>{0..\<tau>}. (\<theta> (x \<tau>) - \<nu> (x \<tau>)) - (\<theta> (x 0) - \<nu> (x 0)) = 
   (\<lambda>\<tau>. \<tau> *\<^sub>R (\<theta>' (x r) -  \<nu>' (x r))) (\<tau> - 0)" 
-    by(rule_tac closed_segment_mvt, auto simp: \<open>0 \<le> \<tau>\<close>)
-  then obtain r where "r \<in> {0--\<tau>}" and 
+    by(rule_tac mvt_very_simple) (auto simp: tHyp)
+  then obtain r where "r \<in> {0..\<tau>}" and 
     "\<theta> (x \<tau>) - \<nu> (x \<tau>) = (\<tau> - 0) *\<^sub>R (\<theta>' (x r) -  \<nu>' (x r)) + (\<theta> (x 0) - \<nu> (x 0))" 
     by force 
   also have "... > 0" 
@@ -431,18 +423,16 @@ proof(simp add: diff_invariant_def ivp_sols_def, clarsimp)
     by simp
 qed
 
-lemma [ode_invariant_rules]:
-fixes \<theta>::"'a::banach \<Rightarrow> real"
-assumes "I1 is_diff_invariant_of f along {0..t}" 
-    and "I2 is_diff_invariant_of f along {0..t}"
-shows "(\<lambda>s. I1 s \<and> I2 s) is_diff_invariant_of f along {0..t}"
+lemma [diff_invariant_rules]:
+assumes "I\<^sub>1 is_diff_invariant_of f along {0..t}" 
+    and "I\<^sub>2 is_diff_invariant_of f along {0..t}"
+shows "(\<lambda>s. I\<^sub>1 s \<and> I\<^sub>2 s) is_diff_invariant_of f along {0..t}"
   using assms unfolding diff_invariant_def by auto
 
-lemma [ode_invariant_rules]:
-fixes \<theta>::"'a::banach \<Rightarrow> real"
-assumes "I1 is_diff_invariant_of f along {0..t}" 
-    and "I2 is_diff_invariant_of f along {0..t}"
-shows "(\<lambda>s. I1 s \<or> I2 s) is_diff_invariant_of f along {0..t}"
+lemma [diff_invariant_rules]:
+assumes "I\<^sub>1 is_diff_invariant_of f along {0..t}" 
+    and "I\<^sub>2 is_diff_invariant_of f along {0..t}"
+shows "(\<lambda>s. I\<^sub>1 s \<or> I\<^sub>2 s) is_diff_invariant_of f along {0..t}"
   using assms unfolding diff_invariant_def by auto
 
 end
