HybridVerifVecs/nd_funs/cat2ndfun.thy
@@ -21,12 +21,10 @@ text\<open> Our semantics correspond now to nondeterministic functions @{typ "'a
 some auxiliary lemmas for them and show that they form an antidomain kleene algebra. The proof just 
 extends the results on the Transformer\_Semantics.Kleisli\_Quantale theory.\<close>
 
-\<comment> \<open>Analog of already existing @{thm Rep_nd_fun_inverse[no_vars]}.\<close>
-lemma Abs_nd_fun_inverse2[simp]:"(f\<^sup>\<bullet>)\<^sub>\<bullet> = f" 
-  by(simp add: Abs_nd_fun_inverse)
+declare Abs_nd_fun_inverse [simp]
 
-\<comment> \<open>Analog of already existing @{thm Rep_nd_fun_inverse[no_vars]}.\<close>
-lemma nd_fun_ext:"(\<And>x. (f\<^sub>\<bullet>) x = (g\<^sub>\<bullet>) x) \<Longrightarrow> f = g"
+\<comment> \<open>Analog of already existing @{thm fun_eq_iff[no_vars]}.\<close>
+lemma nd_fun_ext: "(\<And>x. (f\<^sub>\<bullet>) x = (g\<^sub>\<bullet>) x) \<Longrightarrow> f = g"
   apply(subgoal_tac "Rep_nd_fun f = Rep_nd_fun g")
   using Rep_nd_fun_inject apply blast
   by(rule ext, simp)
@@ -36,32 +34,36 @@ begin
 
 lift_definition antidomain_op_nd_fun :: "'a nd_fun \<Rightarrow> 'a nd_fun" 
   is "\<lambda>f. (\<lambda>x. if ((f\<^sub>\<bullet>) x = {}) then {x} else {})\<^sup>\<bullet>".
+
 lift_definition zero_nd_fun :: "'a nd_fun" 
   is "\<zeta>\<^sup>\<bullet>".
+
 lift_definition star_nd_fun :: "'a nd_fun \<Rightarrow> 'a nd_fun" 
   is "\<lambda>(f::'a nd_fun).qstar f".
+
 lift_definition plus_nd_fun :: "'a nd_fun \<Rightarrow> 'a nd_fun \<Rightarrow> 'a nd_fun" 
   is "\<lambda>f g.((f\<^sub>\<bullet>) \<squnion> (g\<^sub>\<bullet>))\<^sup>\<bullet>".
 
 named_theorems nd_fun_aka "antidomain kleene algebra properties for nondeterministic functions."
 
-lemma nd_fun_assoc[nd_fun_aka]:"(a::'a nd_fun) + b + c = a + (b + c)"
+lemma nd_fun_assoc[nd_fun_aka]: "(a::'a nd_fun) + b + c = a + (b + c)"
   by(transfer, simp add: ksup_assoc)
 
-lemma nd_fun_comm[nd_fun_aka]:"(a::'a nd_fun) + b = b + a"
+lemma nd_fun_comm[nd_fun_aka]: "(a::'a nd_fun) + b = b + a"
   by(transfer, simp add: ksup_comm)
 
-lemma nd_fun_distr[nd_fun_aka]:"((x::'a nd_fun) + y) \<cdot> z = x \<cdot> z + y \<cdot> z"
-  and nd_fun_distl[nd_fun_aka]:"x \<cdot> (y + z) = x \<cdot> y + x \<cdot> z"
+lemma nd_fun_distr[nd_fun_aka]: "((x::'a nd_fun) + y) \<cdot> z = x \<cdot> z + y \<cdot> z"
+  and nd_fun_distl[nd_fun_aka]: "x \<cdot> (y + z) = x \<cdot> y + x \<cdot> z"
   by(transfer, simp add: kcomp_distr, transfer, simp add: kcomp_distl)
 
-lemma nd_fun_zero_sum[nd_fun_aka]:"0 + (x::'a nd_fun) = x" 
-  and nd_fun_zero_dot[nd_fun_aka]:"0 \<cdot> x = 0"
+lemma nd_fun_zero_sum[nd_fun_aka]: "0 + (x::'a nd_fun) = x" 
+  and nd_fun_zero_dot[nd_fun_aka]: "0 \<cdot> x = 0"
   by(transfer, simp, transfer, auto) 
 
-lemma nd_fun_leq[nd_fun_aka]:"((x::'a nd_fun) \<le> y) = (x + y = y)"
-  and nd_fun_leq_add[nd_fun_aka]:" z \<cdot> x \<le> z \<cdot> (x + y)"
-   apply(transfer, metis Abs_nd_fun_inverse2 Rep_nd_fun_inverse le_iff_sup)
+lemma nd_fun_leq[nd_fun_aka]: "((x::'a nd_fun) \<le> y) = (x + y = y)"
+  and nd_fun_leq_add[nd_fun_aka]: " z \<cdot> x \<le> z \<cdot> (x + y)"
+   apply(transfer)
+   apply(metis (no_types, lifting) less_eq_nd_fun.transfer sup.absorb_iff2 sup_nd_fun.transfer)
   by(transfer, simp add: kcomp_isol)
 
 lemma nd_fun_ad_zero[nd_fun_aka]: "ad (x::'a nd_fun) \<cdot> x = 0"
@@ -71,9 +73,9 @@ lemma nd_fun_ad_zero[nd_fun_aka]: "ad (x::'a nd_fun) \<cdot> x = 0"
    apply(transfer, rule nd_fun_ext, simp, simp add: kcomp_def)
   by(transfer, simp, rule nd_fun_ext, simp add: kcomp_def)
 
-lemma nd_star_one[nd_fun_aka]:"1 + (x::'a nd_fun) \<cdot> x\<^sup>\<star> \<le> x\<^sup>\<star>"
-  and nd_star_unfoldl[nd_fun_aka]:"z + x \<cdot> y \<le> y \<Longrightarrow> x\<^sup>\<star> \<cdot> z \<le> y"
-  and nd_star_unfoldr[nd_fun_aka]:"z + y \<cdot> x \<le> y \<Longrightarrow> z \<cdot> x\<^sup>\<star> \<le> y"
+lemma nd_star_one[nd_fun_aka]: "1 + (x::'a nd_fun) \<cdot> x\<^sup>\<star> \<le> x\<^sup>\<star>"
+  and nd_star_unfoldl[nd_fun_aka]: "z + x \<cdot> y \<le> y \<Longrightarrow> x\<^sup>\<star> \<cdot> z \<le> y"
+  and nd_star_unfoldr[nd_fun_aka]: "z + y \<cdot> x \<le> y \<Longrightarrow> z \<cdot> x\<^sup>\<star> \<le> y"
     apply(transfer, metis Abs_nd_fun_inverse Rep_comp_hom UNIV_I fun_star_unfoldr 
       le_sup_iff less_eq_nd_fun.abs_eq mem_Collect_eq one_nd_fun.abs_eq qstar_comm)
    apply(transfer, metis (no_types, lifting) Abs_comp_hom Rep_nd_fun_inverse 
@@ -85,6 +87,7 @@ instance
   apply intro_classes apply auto
   using nd_fun_aka apply simp_all
   by(transfer; auto)+
+
 end
 
 text\<open> Now that we know that nondeterministic functions form an Antidomain Kleene Algebra, we give
@@ -94,39 +97,25 @@ Then we add an operation that does the opposite and prove the relationship betwe
 abbreviation p2ndf :: "'a pred \<Rightarrow> 'a nd_fun" ("(1\<lceil>_\<rceil>)")
   where "\<lceil>Q\<rceil> \<equiv> (\<lambda> x::'a. {s::'a. s = x \<and> Q s})\<^sup>\<bullet>"
 
-lemma le_nd_fun_def:"F\<^sup>\<bullet> \<le> G\<^sup>\<bullet> = (\<forall>s. F s \<subseteq> G s)"
+lemma le_p2ndf_iff[simp]: "\<lceil>P\<rceil> \<le> \<lceil>Q\<rceil> = (\<forall>s. P s \<longrightarrow> Q s)"
   by(transfer, auto simp: le_fun_def)
 
-lemma le_p2ndf_iff[simp]:"\<lceil>P\<rceil> \<le> \<lceil>Q\<rceil> = (\<forall>s. P s \<longrightarrow> Q s)"
-  by(transfer, auto simp: le_fun_def)
-
-lemma eq_p2ndf_iff:"(\<lceil>P\<rceil> = \<lceil>Q\<rceil>) = (P = Q)"
-proof(safe)
-  assume "\<lceil>P\<rceil> = \<lceil>Q\<rceil>"
-  hence "\<lceil>P\<rceil> \<le> \<lceil>Q\<rceil> \<and> \<lceil>Q\<rceil> \<le> \<lceil>P\<rceil>" by simp
-  then have "(\<forall>s. P s \<longrightarrow> Q s) \<and> (\<forall>s. Q s \<longrightarrow> P s)" by simp
-  thus "P = Q" by auto
-qed
-
-lemma p2ndf_le_eta[simp]:"\<lceil>P\<rceil> \<le> \<eta>\<^sup>\<bullet>"
+lemma p2ndf_le_eta[simp]: "\<lceil>P\<rceil> \<le> \<eta>\<^sup>\<bullet>"
   by(transfer, simp add: le_fun_def, clarify)
 
-lemma ads_d_p2ndf[simp]:"d \<lceil>P\<rceil> = \<lceil>P\<rceil>"
+lemma ads_d_p2ndf[simp]: "d \<lceil>P\<rceil> = \<lceil>P\<rceil>"
   unfolding ads_d_def antidomain_op_nd_fun_def by(rule nd_fun_ext, auto)
 
-lemma ad_p2ndf[simp]:"ad \<lceil>P\<rceil> = \<lceil>\<lambda>s. \<not> P s\<rceil>"
+lemma ad_p2ndf[simp]: "ad \<lceil>P\<rceil> = \<lceil>\<lambda>s. \<not> P s\<rceil>"
   unfolding antidomain_op_nd_fun_def by(rule nd_fun_ext, auto)
 
 abbreviation ndf2p :: "'a nd_fun \<Rightarrow> 'a \<Rightarrow> bool" ("(1\<lfloor>_\<rfloor>)")
   where "\<lfloor>f\<rfloor> \<equiv> (\<lambda>x. x \<in> Domain (\<R> (f\<^sub>\<bullet>)))"
 
-lemma p2ndf_ndf2p_id:"F \<le> \<eta>\<^sup>\<bullet> \<Longrightarrow> \<lceil>\<lfloor>F\<rfloor>\<rceil> = F"
+lemma p2ndf_ndf2p_id: "F \<le> \<eta>\<^sup>\<bullet> \<Longrightarrow> \<lceil>\<lfloor>F\<rfloor>\<rceil> = F"
   unfolding f2r_def apply(rule nd_fun_ext)
   apply(subgoal_tac "\<forall>x. (F\<^sub>\<bullet>) x \<subseteq> {x}", simp)
   by(blast, simp add: le_fun_def less_eq_nd_fun.rep_eq)
-
-lemma ndf2p_p2ndf_id:"\<lfloor>\<lceil>P\<rceil>\<rfloor> = P"
-  by(simp add: f2r_def)
 
 section\<open> Verification of regular programs \<close>
 
@@ -136,19 +125,19 @@ we explore its behavior with the previously defined lifting ($\lceil-\rceil$*) a
 
 abbreviation "wp f \<equiv> fbox (f::'a nd_fun)"
 
-lemma wp_eta[simp]:"wp (\<eta>\<^sup>\<bullet>) \<lceil>P\<rceil> = \<lceil>P\<rceil>"
+lemma wp_eta[simp]: "wp (\<eta>\<^sup>\<bullet>) \<lceil>P\<rceil> = \<lceil>P\<rceil>"
   apply(simp add: fbox_def, transfer, simp)
   by(rule nd_fun_ext, auto simp: kcomp_def)
 
-lemma wp_nd_fun:"wp (F\<^sup>\<bullet>) \<lceil>P\<rceil> = \<lceil>\<lambda> x. \<forall> y. y \<in> (F x) \<longrightarrow> P y\<rceil>"
+lemma wp_nd_fun: "wp (F\<^sup>\<bullet>) \<lceil>P\<rceil> = \<lceil>\<lambda> x. \<forall> y. y \<in> (F x) \<longrightarrow> P y\<rceil>"
   apply(simp add: fbox_def, transfer, simp)
   by(rule nd_fun_ext, auto simp: kcomp_def)
 
-lemma wp_nd_fun2:"wp F \<lceil>P\<rceil> = \<lceil>\<lambda> x. \<forall> y. y \<in> ((F\<^sub>\<bullet>) x) \<longrightarrow> P y\<rceil>"
+lemma wp_nd_fun2: "wp F \<lceil>P\<rceil> = \<lceil>\<lambda> x. \<forall> y. y \<in> ((F\<^sub>\<bullet>) x) \<longrightarrow> P y\<rceil>"
   apply(simp add: fbox_def antidomain_op_nd_fun_def)
   by(rule nd_fun_ext, auto simp: Rep_comp_hom kcomp_prop)
 
-lemma wp_nd_fun_etaD:"wp (F\<^sup>\<bullet>) \<lceil>P\<rceil> = \<eta>\<^sup>\<bullet> \<Longrightarrow>  (\<forall>y. y \<in> (F x) \<longrightarrow> P y)"
+lemma wp_nd_fun_etaD: "wp (F\<^sup>\<bullet>) \<lceil>P\<rceil> = \<eta>\<^sup>\<bullet> \<Longrightarrow>  (\<forall>y. y \<in> (F x) \<longrightarrow> P y)"
 proof
   fix y assume "wp (F\<^sup>\<bullet>) \<lceil>P\<rceil> = (\<eta>\<^sup>\<bullet>)"
   from this have "\<eta>\<^sup>\<bullet> = \<lceil>\<lambda>s. \<forall>y. s2p (F s) y \<longrightarrow> P y\<rceil>" 
@@ -159,12 +148,9 @@ proof
   then show "s2p (F x) y \<longrightarrow> P y" by auto
 qed
 
-lemma p2ndf_ndf2p_wp:"\<lceil>\<lfloor>wp R P\<rfloor>\<rceil> = wp R P"
+lemma p2ndf_ndf2p_wp: "\<lceil>\<lfloor>wp R P\<rfloor>\<rceil> = wp R P"
   apply(rule p2ndf_ndf2p_id)
-  by (simp add: a_subid fbox_def one_nd_fun.transfer) 
-
-lemma p2ndf_ndf2p_wp_sym:"wp R P = \<lceil>\<lfloor>wp R P\<rfloor>\<rceil>"
-  by(rule sym, simp add: p2ndf_ndf2p_wp)
+  by (simp add: a_subid fbox_def one_nd_fun.transfer)
 
 lemma ndf2p_wpD: "\<lfloor>wp F \<lceil>Q\<rceil>\<rfloor> s = (\<forall>s'. s' \<in> (F\<^sub>\<bullet>) s \<longrightarrow> Q s')"  
   apply(subgoal_tac "F = (F\<^sub>\<bullet>)\<^sup>\<bullet>")
@@ -175,13 +161,13 @@ lemma ndf2p_wpD: "\<lfloor>wp F \<lceil>Q\<rceil>\<rfloor> s = (\<forall>s'. s' 
 text\<open> We can verify that our introduction of @{text "wp"} coincides with another definition of the 
 forward box operator @{thm ffb_def[no_vars]} with the following characterization lemmas. \<close>
 
-lemma ffb_is_wp:"fb\<^sub>\<F> (F\<^sub>\<bullet>) {x. P x} = {s. \<lfloor>wp F \<lceil>P\<rceil>\<rfloor> s}"
+lemma ffb_is_wp: "fb\<^sub>\<F> (F\<^sub>\<bullet>) {x. P x} = {s. \<lfloor>wp F \<lceil>P\<rceil>\<rfloor> s}"
   unfolding ffb_def unfolding map_dual_def klift_def kop_def fbox_def
   unfolding r2f_def f2r_def apply clarsimp
   unfolding antidomain_op_nd_fun_def unfolding dual_set_def 
   unfolding times_nd_fun_def kcomp_def by force
 
-lemma wp_is_ffb:"wp F P = (\<lambda>x. {x} \<inter> fb\<^sub>\<F> (F\<^sub>\<bullet>) {s. \<lfloor>P\<rfloor> s})\<^sup>\<bullet>"
+lemma wp_is_ffb: "wp F P = (\<lambda>x. {x} \<inter> fb\<^sub>\<F> (F\<^sub>\<bullet>) {s. \<lfloor>P\<rfloor> s})\<^sup>\<bullet>"
   apply(rule nd_fun_ext, simp)
   unfolding ffb_def unfolding map_dual_def klift_def kop_def fbox_def
   unfolding r2f_def f2r_def apply clarsimp
@@ -191,13 +177,13 @@ lemma wp_is_ffb:"wp F P = (\<lambda>x. {x} \<inter> fb\<^sub>\<F> (F\<^sub>\<bul
 
 text\<open> Next, we introduce assignments and compute their @{text "wp"}. \<close>
 
-abbreviation vec_upd :: "('a^'b) \<Rightarrow> 'b \<Rightarrow> 'a \<Rightarrow> 'a^'b" ("_(2[_ :== _])" [70, 65] 61) where 
-"x[i :== a] \<equiv> (\<chi> j. (if j = i then a else (x $ j)))"
+abbreviation vec_upd :: "('a^'b) \<Rightarrow> 'b \<Rightarrow> 'a \<Rightarrow> 'a^'b"
+  where "vec_upd x i a \<equiv> vec_lambda ((vec_nth x)(i := a))"
 
-abbreviation assign :: "'b \<Rightarrow> ('a^'b \<Rightarrow> 'a) \<Rightarrow> ('a^'b) nd_fun" ("(2[_ ::== _])" [70, 65] 61) where 
-"[x ::== expr]\<equiv> (\<lambda>s. {s[x :== expr s]})\<^sup>\<bullet>" 
+abbreviation assign :: "'b \<Rightarrow> ('a^'b \<Rightarrow> 'a) \<Rightarrow> ('a^'b) nd_fun" ("(2_ ::= _)" [70, 65] 61) 
+  where "(x ::= e)\<equiv> (\<lambda>s. {vec_upd s x (e s)})\<^sup>\<bullet>" 
 
-lemma wp_assign[simp]: "wp ([x ::== expr]) \<lceil>Q\<rceil> = \<lceil>\<lambda>s. Q (s[x :== expr s])\<rceil>"
+lemma wp_assign[simp]: "wp (x ::= e) \<lceil>Q\<rceil> = \<lceil>\<lambda>s. Q (vec_upd s x (e s))\<rceil>"
   by(subst wp_nd_fun, rule nd_fun_ext, simp)
 
 text\<open> The @{text "wp"} of the composition was already obtained in KAD.Antidomain\_Semiring:
@@ -206,11 +192,10 @@ text\<open> The @{text "wp"} of the composition was already obtained in KAD.Anti
 text\<open> We also have an implementation of the conditional operator and its @{text "wp"}. \<close>
 
 definition (in antidomain_kleene_algebra) cond :: "'a \<Rightarrow> 'a \<Rightarrow> 'a \<Rightarrow> 'a" 
-("if _ then _ else _ fi" [64,64,64] 63) where "if p then x else y fi = d p \<cdot> x + ad p \<cdot> y"
+  ("if _ then _ else _ fi" [64,64,64] 63) where "if p then x else y fi = d p \<cdot> x + ad p \<cdot> y"
 
 abbreviation cond_sugar :: "'a pred \<Rightarrow> 'a nd_fun \<Rightarrow> 'a nd_fun \<Rightarrow> 'a nd_fun" 
-("IF _ THEN _ ELSE _ FI" [64,64,64] 63) where
-  "IF P THEN X ELSE Y FI \<equiv> cond \<lceil>P\<rceil> X Y"
+  ("IF _ THEN _ ELSE _ FI" [64,64,64] 63) where "IF P THEN X ELSE Y FI \<equiv> cond \<lceil>P\<rceil> X Y"
 
 lemma wp_if_then_else:
   assumes "\<lceil>\<lambda>s. P s \<and> T s\<rceil> \<le> wp X \<lceil>Q\<rceil>"
@@ -224,13 +209,9 @@ lemma wp_if_then_else:
 text\<open> Finally we also deal with finite iteration. \<close>
 
 lemma (in antidomain_kleene_algebra) fbox_starI: 
-assumes "d p \<le> d i" and "d i \<le> |x] i" and "d i \<le> d q"
-shows "d p \<le> |x\<^sup>\<star>] q"
+  assumes "d p \<le> d i" and "d i \<le> |x] i" and "d i \<le> d q"
+  shows "d p \<le> |x\<^sup>\<star>] q"
   by (meson assms local.dual_order.trans local.fbox_iso local.fbox_star_induct_var)
-
-lemma nd_fun_ads_d_def:"d (f::'a nd_fun) = (\<lambda>x. if (f\<^sub>\<bullet>) x = {} then {} else \<eta> x )\<^sup>\<bullet>"
-  unfolding ads_d_def apply(rule nd_fun_ext, simp)
-  apply transfer by auto
 
 lemma ads_d_mono: "x \<le> y \<Longrightarrow> d x \<le> d y"
   by (metis ads_d_def fbox_antitone_var fbox_dom)
@@ -242,19 +223,19 @@ lemma nd_fun_top_ads_d:"(x::'a nd_fun) \<le> 1 \<Longrightarrow> d x = x"
   by auto
 
 lemma wp_starI:
-assumes "P \<le> I" and "I \<le> wp F I" and "I \<le> Q"
-shows "P \<le> wp (qstar F) Q"
+  assumes "P \<le> I" and "I \<le> wp F I" and "I \<le> Q"
+  shows "P \<le> wp (qstar F) Q"
 proof-
-  from assms(1,2) have "P \<le> 1"
-    by (metis a_subid basic_trans_rules(23) fbox_def) 
+  have "P \<le> 1"
+    using assms(1,2) by (metis a_subid basic_trans_rules(23) fbox_def) 
   hence "d P = P" using nd_fun_top_ads_d by blast
   have "\<And> x y. d (wp x y) = wp x y"
     by(metis ds.ddual.mult_oner fbox_mult fbox_one)
-  from this and assms have "d P \<le> d I \<and> d I \<le> wp F I \<and> d I \<le> d Q"
-    by (metis (no_types) ads_d_mono assms)
+  hence "d P \<le> d I \<and> d I \<le> wp F I \<and> d I \<le> d Q"
+    using assms by (metis (no_types) ads_d_mono assms)
   hence "d P \<le> wp (F\<^sup>\<star>) Q"
     by(simp add: fbox_starI[of _ I])
-  then show "P \<le> wp (qstar F) Q"
+  thus "P \<le> wp (qstar F) Q"
     using \<open>d P = P\<close> by (transfer, simp)
 qed
 
@@ -279,25 +260,18 @@ lemma ivp_solsD:
     and "x t\<^sub>0 = s" and "t\<^sub>0 \<in> T"
   using assms unfolding ivp_sols_def by auto
 
-lemma "(t::real) \<in> {0--t}"
-  by (rule ends_in_segment(2))
-
-lemma "(t::real) \<in> {0..t}"
-  apply auto
-  oops
-
-definition "g_orbital f T t\<^sub>0 G s = \<Union> {{x t|t. t \<in> T \<and> G \<rhd> x {t\<^sub>0--t} }|x. x \<in> ivp_sols f T t\<^sub>0 s}"
+definition "g_orbital f T t\<^sub>0 G s = \<Union> {{x t|t. t \<in> T \<and> G \<rhd> x {t\<^sub>0..t} }|x. x \<in> ivp_sols f T t\<^sub>0 s}"
 
 lemma g_orbital_eq: "g_orbital f T t\<^sub>0 G s = 
-  {x t |t x. t \<in> T \<and> (D x = (f \<circ> x) on T) \<and> x t\<^sub>0 = s \<and> t\<^sub>0 \<in> T \<and> G \<rhd> x {t\<^sub>0--t}}"
+  {x t |t x. t \<in> T \<and> (D x = (f \<circ> x) on T) \<and> x t\<^sub>0 = s \<and> t\<^sub>0 \<in> T \<and> G \<rhd> x {t\<^sub>0..t}}"
   unfolding g_orbital_def ivp_sols_def by auto
 
-lemma "g_orbital f T t\<^sub>0 G s = (\<Union> x \<in> ivp_sols f T t\<^sub>0 s. {x t|t. t \<in> T \<and> G \<rhd> x {t\<^sub>0--t}})"
+lemma "g_orbital f T t\<^sub>0 G s = (\<Union> x \<in> ivp_sols f T t\<^sub>0 s. {x t|t. t \<in> T \<and> G \<rhd> x {t\<^sub>0..t}})"
   unfolding g_orbital_def ivp_sols_def by auto
 
 lemma g_orbitalI:
   assumes "D x = (f \<circ> x) on T" "x t\<^sub>0 = s"
-    and "t\<^sub>0 \<in> T" "t \<in> T" and "G \<rhd> x {t\<^sub>0--t}"
+    and "t\<^sub>0 \<in> T" "t \<in> T" and "G \<rhd> x {t\<^sub>0..t}"
   shows "x t \<in> g_orbital f T t\<^sub>0 G s"
   using assms unfolding g_orbital_def ivp_sols_def by blast
 
@@ -305,7 +279,7 @@ lemma g_orbitalD:
   assumes "s' \<in> g_orbital f T t\<^sub>0 G s"
   obtains x and t where "x \<in> ivp_sols f T t\<^sub>0 s" 
   and "D x = (f \<circ> x) on T" "x t\<^sub>0 = s"
-  and "x t = s'" and "t\<^sub>0 \<in> T" "t \<in> T" and "G \<rhd> x {t\<^sub>0--t}"
+  and "x t = s'" and "t\<^sub>0 \<in> T" "t \<in> T" and "G \<rhd> x {t\<^sub>0..t}"
   using assms unfolding g_orbital_def ivp_sols_def by blast
 
 abbreviation g_evol ::"(('a::banach)\<Rightarrow>'a) \<Rightarrow> real set \<Rightarrow> 'a pred \<Rightarrow> 'a nd_fun" ("(1[x\<acute>=_]_ & _)") 
@@ -326,25 +300,27 @@ lemma orbit_eq[simp]: "orbit s = {\<phi> t s| t. t \<in> T}"
   by(auto intro: usolves_ivp intro!: ivp simp: init_time)
 
 lemma g_evol_collapses: 
-  shows "([x\<acute>=f]T & G) = (\<lambda>s. {\<phi> t s| t. t \<in> T \<and> G \<rhd> (\<lambda>r. \<phi> r s) {0--t}})\<^sup>\<bullet>"
+  shows "([x\<acute>=f]T & G) = (\<lambda>s. {\<phi> t s| t. t \<in> T \<and> G \<rhd> (\<lambda>r. \<phi> r s) {0..t}})\<^sup>\<bullet>"
 proof(rule nd_fun_ext, rule subset_antisym, simp_all add: subset_eq)
   fix s
-  let "?P s s'" = "\<exists>t. s' = \<phi> t s \<and> s2p T t \<and> (\<forall>r\<in>{0--t}. G (\<phi> r s))"
+  let "?P s s'" = "\<exists>t. s' = \<phi> t s \<and> s2p T t \<and> (\<forall>r\<in>{0..t}. G (\<phi> r s))"
   {fix s' assume "s' \<in> g_orbital f T 0 G s"
-    then obtain x and t where x_ivp:"D x = (f \<circ> x) on T" 
-      "x 0 = s" and "x t = s'" and "t \<in> T" and guard:"G \<rhd> x {0--t}"
-      unfolding g_orbital_eq by blast
-    hence obs:"\<forall>\<tau>\<in>{0--t}. x \<tau> = \<phi> \<tau> s"
-      using usolves_ivp[of x s] closed_segment_subset_domainI init_time comp_def
-      by (metis (mono_tags, lifting) has_vderiv_eq)
-    hence "G \<rhd> (\<lambda>r. \<phi> r s) {0--t}"
+    then obtain x and t where x_ivp:"D x = (\<lambda>t. f (x t)) on T"
+      "x 0 = s" and "x t = s'" and "t \<in> T" and guard:"G \<rhd> x {0..t}"
+      unfolding g_orbital_eq by auto
+    hence obs:"\<forall>\<tau>\<in>{0..t}. x \<tau> = \<phi> \<tau> s"
+      using usolves_ivp[OF x_ivp]
+      by (meson atLeastAtMost_iff init_time interval mem_is_interval_1_I)
+    hence "G \<rhd> (\<lambda>r. \<phi> r s) {0..t}"
       using guard by simp
-    hence "\<exists>t. s' = \<phi> t s \<and> s2p T t \<and> (\<forall>r\<in>{0--t}. G (\<phi> r s))"
-      using \<open>x t = s'\<close> \<open>t \<in> T\<close> obs by blast}
+    also have "\<phi> t s = x t"
+      using usolves_ivp x_ivp \<open>t \<in> T\<close> by simp
+    ultimately have "\<exists>t. s' = \<phi> t s \<and> s2p T t \<and> (\<forall>r\<in>{0..t}. G (\<phi> r s))"
+      using \<open>x t = s'\<close> \<open>t \<in> T\<close> by auto}
   thus "\<forall>s'\<in>g_orbital f T 0 G s. ?P s s'"
     by blast
-  {fix s' assume "\<exists>t. s' = \<phi> t s \<and> s2p T t \<and> (\<forall>r\<in>{0--t}. G (\<phi> r s))"
-    then obtain t where "G \<rhd> (\<lambda>r. \<phi> r s) {0--t}" and "t \<in> T" and "\<phi> t s = s'"
+  {fix s' assume "\<exists>t. s' = \<phi> t s \<and> s2p T t \<and> (\<forall>r\<in>{0..t}. G (\<phi> r s))"
+    then obtain t where "G \<rhd> (\<lambda>r. \<phi> r s) {0..t}" and "t \<in> T" and "\<phi> t s = s'"
       by blast
     hence "s' \<in> g_orbital f T 0 G s"
       by(auto intro: g_orbitalI simp: ivp init_time)}
@@ -355,13 +331,15 @@ qed
 lemma wp_orbit: "wp ((\<lambda> s. orbit s)\<^sup>\<bullet>) \<lceil>Q\<rceil> = \<lceil>\<lambda> s. \<forall> t \<in> T. Q (\<phi> t s)\<rceil>"
   unfolding orbit_eq wp_nd_fun apply(rule nd_fun_ext) by auto
 
-lemma wp_g_orbit: "wp ([x\<acute>=f]T & G) \<lceil>Q\<rceil> = \<lceil>\<lambda> s. \<forall>t\<in>T. (G \<rhd> (\<lambda>r. \<phi> r s) {0--t}) \<longrightarrow> Q (\<phi> t s)\<rceil>"
+lemma wp_g_orbit: "wp ([x\<acute>=f]T & G) \<lceil>Q\<rceil> = \<lceil>\<lambda> s. \<forall>t\<in>T. (G \<rhd> (\<lambda>r. \<phi> r s) {0..t}) \<longrightarrow> Q (\<phi> t s)\<rceil>"
   unfolding g_evol_collapses wp_nd_fun apply(rule nd_fun_ext) by auto
 
 end
 
-lemma (in global_flow) ivp_sols_collapse[simp]: "ivp_sols f UNIV 0 s = {(\<lambda>t. \<phi> t s)}"
-  by(auto intro: usolves_ivp simp: ivp_sols_def ivp)
+lemma (in local_flow) ivp_sols_collapse: "ivp_sols f T 0 s = {(\<lambda>t. \<phi> t s)}"
+  apply(auto simp: ivp_sols_def ivp init_time fun_eq_iff)
+  apply(rule unique_solution, simp_all add: ivp)
+  oops
 
 text\<open> The previous lemma allows us to compute wlps for known systems of ODEs. We can also implement
 a version of it as an inference rule. A simple computation of a wlp is shown immmediately after.\<close>
@@ -370,8 +348,7 @@ lemma dSolution:
   assumes "local_flow f T L \<phi>"
     and "\<forall>s. P s \<longrightarrow> (\<forall> t \<in> T. (G \<rhd> (\<lambda>r. \<phi> r s) {0..t}) \<longrightarrow> Q (\<phi> t s))"
   shows "\<lceil>P\<rceil> \<le> wp ([x\<acute>=f]T & G) \<lceil>Q\<rceil>"
-  using assms apply(subst local_flow.wp_g_orbit, auto)
-  by (simp add: Starlike.closed_segment_eq_real_ivl)
+  using assms by(subst local_flow.wp_g_orbit, auto)
 
 lemma line_DS: "0 \<le> t \<Longrightarrow> wp ([x\<acute>=\<lambda>s. c]{0..t} & G) \<lceil>Q\<rceil> = 
     \<lceil>\<lambda> x. \<forall> \<tau> \<in> {0..t}. (G \<rhd> (\<lambda>r. x + r *\<^sub>R c) {0..\<tau>}) \<longrightarrow> Q (x + \<tau> *\<^sub>R c)\<rceil>"
@@ -387,24 +364,23 @@ Then we prove the inference rules which are used in verification proofs.\<close>
 
 subsubsection\<open> Differential Weakening \<close>
         
-lemma DW: "wp ([x\<acute>=f]T & G) \<lceil>Q\<rceil> = wp ([x\<acute>=f]T & G) \<lceil>\<lambda> s. G s \<longrightarrow> Q s\<rceil>"
-  apply(subst wp_nd_fun)+
+lemma DW: "wp ([x\<acute>=f]{0..t} & G) \<lceil>Q\<rceil> = wp ([x\<acute>=f]{0..t} & G) \<lceil>\<lambda> s. G s \<longrightarrow> Q s\<rceil>"
   apply(rule nd_fun_ext)
-  by(auto simp: g_orbital_eq)
+  by (auto intro: g_orbitalD simp: wp_nd_fun)
 
 lemma dWeakening: 
   assumes "\<lceil>G\<rceil> \<le> \<lceil>Q\<rceil>"
-  shows "\<lceil>P\<rceil> \<le> wp ([x\<acute>=f]T & G) \<lceil>Q\<rceil>"
+  shows "\<lceil>P\<rceil> \<le> wp ([x\<acute>=f]{0..t} & G) \<lceil>Q\<rceil>"
   using assms apply(subst wp_nd_fun)
-  by(auto simp: le_fun_def g_orbital_eq)
+  by(auto simp: g_evol_def)
 
 subsubsection\<open> Differential Cut \<close>
 
 lemma wp_g_orbit_etaD:
-  assumes "wp ([x\<acute>=f]T & G) \<lceil>C\<rceil> = \<eta>\<^sup>\<bullet>" and "\<forall> r\<in>{0--t}. x r \<in> g_orbital f T 0 G s"
-  shows "\<forall>r\<in>{0--t}. C (x r)"
+  assumes "wp ([x\<acute>=f]T & G) \<lceil>C\<rceil> = \<eta>\<^sup>\<bullet>" and "\<forall> r\<in>{0..t}. x r \<in> g_orbital f T 0 G s"
+  shows "\<forall>r\<in>{0..t}. C (x r)"
 proof
-  fix r assume "r \<in> {0--t}"
+  fix r assume "r \<in> {0..t}"
   then have "x r \<in> g_orbital f T 0 G s" 
     using assms(2) by blast
   also have "\<forall>y. y \<in> (g_orbital f T 0 G s) \<longrightarrow> C y" 
@@ -419,15 +395,15 @@ proof(rule_tac f="\<lambda> x. wp x \<lceil>Q\<rceil>" in HOL.arg_cong, rule nd_
   fix s
   {fix s' assume "s' \<in> g_orbital f T 0 G s"
     then obtain t::real and x where x_ivp: "D x = (f \<circ> x) on T" "x 0 = s"
-      and guard_x:"G \<rhd> x {0--t}" and "s' = x t" and "0 \<in> T" "t \<in> T"
+      and guard_x:"G \<rhd> x {0..t}" and "s' = x t" and "0 \<in> T" "t \<in> T"
       using g_orbitalD[of s' "f" T 0 G s] by (metis (full_types))
-    from guard_x have "\<forall>r\<in>{0--t}.\<forall> \<tau>\<in>{0--r}. G (x \<tau>)"
-      by (metis contra_subsetD ends_in_segment(1) subset_segment(1))
-    also have "\<forall>\<tau>\<in>{0--t}. \<tau> \<in> T"
-      using interval.closed_segment_subset_domain[OF assms(1) \<open>0 \<in> T\<close> \<open>t \<in> T\<close>] by blast
-    ultimately have "\<forall>\<tau>\<in>{0--t}. x \<tau> \<in> g_orbital f T 0 G s"
+    from guard_x have "\<forall>r\<in>{0..t}.\<forall> \<tau>\<in>{0..r}. G (x \<tau>)"
+      by auto
+    also have "\<forall>\<tau>\<in>{0..t}. \<tau> \<in> T"
+      by (meson \<open>0 \<in> T\<close> \<open>t \<in> T\<close> assms(1) atLeastAtMost_iff interval.interval mem_is_interval_1_I) 
+    ultimately have "\<forall>\<tau>\<in>{0..t}. x \<tau> \<in> g_orbital f T 0 G s"
       using g_orbitalI[OF x_ivp \<open>0 \<in> T\<close>] by blast
-    hence "C \<rhd> x {0--t}" 
+    hence "C \<rhd> x {0..t}" 
       using wp_g_orbit_etaD assms(2) by blast
     hence "s' \<in> g_orbital f T 0 (\<lambda>s. G s \<and> C s) s"
       using g_orbitalI[OF x_ivp \<open>0 \<in> T\<close> \<open>t \<in> T\<close>] guard_x \<open>s' = x t\<close> by fastforce}
@@ -443,12 +419,12 @@ lemma dCut:
   shows "\<lceil>P\<rceil> \<le> wp ([x\<acute>=f]{0..t} & G) \<lceil>Q\<rceil>"
 proof(simp add: wp_nd_fun g_orbital_eq, clarsimp)
   fix \<tau>::real and x::"real \<Rightarrow> 'a" assume "P (x 0)" and "0 \<le> \<tau>" and "\<tau> \<le> t"
-    and x_solves:"D x = (\<lambda>t. f (x t)) on {0..t}" and guard_x:"(\<forall> r \<in> {0--\<tau>}. G (x r))"
-  hence "\<forall>r\<in>{0--\<tau>}.\<forall>\<tau>\<in>{0--r}. G (x \<tau>)"
-    using closed_segment_closed_segment_subset by blast
-  hence "\<forall>r\<in>{0--\<tau>}. x r \<in> g_orbital f {0..t} 0 G (x 0)"
+    and x_solves:"D x = (\<lambda>t. f (x t)) on {0..t}" and guard_x:"(\<forall> r \<in> {0..\<tau>}. G (x r))"
+  hence "\<forall>r\<in>{0..\<tau>}.\<forall>\<tau>\<in>{0..r}. G (x \<tau>)"
+    by auto
+  hence "\<forall>r\<in>{0..\<tau>}. x r \<in> g_orbital f {0..t} 0 G (x 0)"
     using g_orbitalI x_solves \<open>0 \<le> \<tau>\<close> \<open>\<tau> \<le> t\<close> closed_segment_eq_real_ivl by fastforce 
-  hence "\<forall>r\<in>{0--\<tau>}. C (x r)" 
+  hence "\<forall>r\<in>{0..\<tau>}. C (x r)" 
     using wp_C \<open>P (x 0)\<close> by(subst (asm) wp_nd_fun, auto)
   hence "x \<tau> \<in> g_orbital f {0..t} 0 (\<lambda>s. G s \<and> C s) (x 0)"
     using g_orbitalI x_solves guard_x \<open>0 \<le> \<tau>\<close> \<open>\<tau> \<le> t\<close> by fastforce
@@ -467,7 +443,7 @@ lemma DI_sufficiency:
   apply(erule_tac x="s" in allE, clarify)
   by(rule_tac x="0" in exI, rule_tac x=x in exI, auto)
 
-lemma (in local_flow) DI_necessity: (* Not true... check Bohrer formalisation *)
+lemma (in local_flow) DI_necessity:
   shows "wp \<lceil>G\<rceil> \<lceil>Q\<rceil> \<le> wp ([x\<acute>=f]T & G) \<lceil>Q\<rceil>"
   unfolding wp_g_orbit apply(subst wp_nd_fun, clarsimp, safe)
    apply(erule_tac x="0" in ballE)
@@ -475,8 +451,8 @@ lemma (in local_flow) DI_necessity: (* Not true... check Bohrer formalisation *)
   oops
 
 definition diff_invariant :: "'a pred \<Rightarrow> (('a::real_normed_vector) \<Rightarrow> 'a) \<Rightarrow> real set \<Rightarrow> bool" 
-("(_)/ is'_diff'_invariant'_of (_)/ along (_)" [70,65]61) 
-where "I is_diff_invariant_of f along T \<equiv> 
+  ("(_)/ is'_diff'_invariant'_of (_)/ along (_)" [70,65]61) 
+  where "I is_diff_invariant_of f along T \<equiv> 
   (\<forall>s. I s \<longrightarrow> (\<forall> x. x \<in> ivp_sols f T 0 s \<longrightarrow> (\<forall> t \<in> T. I (x t))))"
 
 lemma invariant_to_set:
@@ -488,7 +464,6 @@ lemma invariant_to_set:
   apply(drule mp, simp_all add: subset_eq)
   apply(erule_tac x="xa t" in allE)
   by(drule mp, auto)
-
 
 lemma dInvariant:
   assumes "I is_diff_invariant_of f along T"
@@ -510,61 +485,61 @@ lemma dI:
 
 text\<open> Finally, we obtain some conditions to prove specific instances of differential invariants. \<close>
 
-named_theorems ode_invariant_rules "compilation of rules for differential invariants."
+named_theorems diff_invariant_rules "compilation of rules for differential invariants."
 
-lemma [ode_invariant_rules]:
-fixes \<theta>::"'a::banach \<Rightarrow> real"
-assumes "\<forall> x. (D x = (\<lambda>\<tau>. f (x \<tau>)) on {0..t}) \<longrightarrow> (\<forall> \<tau> \<in> {0..t}. \<forall> r \<in> {0--\<tau>}. 
-  ((\<lambda>\<tau>. \<theta> (x \<tau>) - \<nu> (x \<tau>) ) has_derivative (\<lambda>\<tau>.  \<tau> *\<^sub>R 0)) (at r within {0--\<tau>}))"
-shows "(\<lambda>s. \<theta> s = \<nu> s) is_diff_invariant_of f along {0..t}"
+lemma [diff_invariant_rules]:
+  fixes \<theta>::"'a::banach \<Rightarrow> real"
+  assumes "\<forall>x. (D x = (\<lambda>\<tau>. f (x \<tau>)) on {0..t}) \<longrightarrow> 
+  (\<forall>\<tau>\<in>{0..t}. (D (\<lambda>\<tau>. \<theta> (x \<tau>) - \<nu> (x \<tau>)) = ((*\<^sub>R) 0) on {0..\<tau>}))"
+  shows "(\<lambda>s. \<theta> s = \<nu> s) is_diff_invariant_of f along {0..t}"
 proof(simp add: diff_invariant_def ivp_sols_def, clarsimp)
   fix x \<tau> assume tHyp:"0 \<le> \<tau>" "\<tau> \<le> t" 
     and x_ivp:"D x = (\<lambda>\<tau>. f (x \<tau>)) on {0..t}" "\<theta> (x 0) = \<nu> (x 0)" 
-  hence "\<forall> r \<in> {0--\<tau>}. D (\<lambda>\<tau>. \<theta> (x \<tau>) - \<nu> (x \<tau>)) \<mapsto> (\<lambda>\<tau>. \<tau> *\<^sub>R 0) at r within {0--\<tau>}" 
-    using assms by auto
-  hence "\<exists>r\<in>{0--\<tau>}. (\<theta> (x \<tau>) - \<nu> (x \<tau>)) - (\<theta> (x 0) - \<nu> (x 0)) = (\<lambda>\<tau>. \<tau> *\<^sub>R 0) (\<tau> - 0)" 
-    by(rule_tac closed_segment_mvt, auto simp: tHyp) 
+  hence "\<forall> t \<in> {0..\<tau>}. D (\<lambda>\<tau>. \<theta> (x \<tau>) - \<nu> (x \<tau>)) \<mapsto> (\<lambda>\<tau>. \<tau> *\<^sub>R 0) at t within {0..\<tau>}" 
+    using assms by (auto simp: has_vderiv_on_def has_vector_derivative_def)
+  hence "\<exists>t\<in>{0..\<tau>}. \<theta> (x \<tau>) - \<nu> (x \<tau>) - (\<theta> (x 0) - \<nu> (x 0)) = (\<tau> - 0) \<cdot> 0" 
+    by(rule_tac mvt_very_simple) (auto simp: tHyp)
   thus "\<theta> (x \<tau>) = \<nu> (x \<tau>)" by (simp add: x_ivp(2))
 qed
 
-lemma [ode_invariant_rules]:
-fixes \<theta>::"'a::banach \<Rightarrow> real"
-assumes "\<forall> x. (D x = (\<lambda>\<tau>. f (x \<tau>)) on {0..t}) \<longrightarrow> (\<forall> \<tau> \<in> {0..t}. \<forall> r \<in> {0--\<tau>}. \<theta>' (x r) \<ge> \<nu>' (x r)
-\<and> (D (\<lambda>\<tau>. \<theta> (x \<tau>) - \<nu> (x \<tau>)) \<mapsto> (\<lambda>\<tau>. \<tau> *\<^sub>R (\<theta>' (x r) - \<nu>' (x r))) at r within {0--\<tau>}))"
-shows "(\<lambda>s. \<nu> s \<le> \<theta> s) is_diff_invariant_of f along {0..t}"
+lemma [diff_invariant_rules]:
+  fixes \<theta>::"'a::banach \<Rightarrow> real"
+  assumes "\<forall> x. (D x = (\<lambda>\<tau>. f (x \<tau>)) on {0..t}) \<longrightarrow> (\<forall>\<tau>\<in>{0..t}. \<theta>' (x \<tau>) \<ge> \<nu>' (x \<tau>) \<and> 
+  (D (\<lambda>\<tau>. \<theta> (x \<tau>) - \<nu> (x \<tau>)) = (\<lambda>r. \<theta>' (x r) - \<nu>' (x r)) on {0..\<tau>}))"
+  shows "(\<lambda>s. \<nu> s \<le> \<theta> s) is_diff_invariant_of f along {0..t}"
 proof(simp add: diff_invariant_def ivp_sols_def, clarsimp)
   fix x \<tau> assume tHyp:"0 \<le> \<tau>" "\<tau> \<le> t" 
     and x_ivp:"D x = (\<lambda>\<tau>. f (x \<tau>)) on {0..t}" "\<nu> (x 0) \<le> \<theta> (x 0)"
-  hence primed:"\<forall> r \<in> {0--\<tau>}. (D (\<lambda>\<tau>. \<theta> (x \<tau>) - \<nu> (x \<tau>)) \<mapsto> (\<lambda>\<tau>. \<tau> *\<^sub>R (\<theta>' (x r) - \<nu>' (x r))) 
-  at r within {0--\<tau>}) \<and> \<nu>' (x r) \<le> \<theta>' (x r)" 
-    using assms by auto
-  hence "\<exists>r\<in>{0--\<tau>}. (\<theta> (x \<tau>) - \<nu> (x \<tau>)) - (\<theta> (x 0) - \<nu> (x 0)) = 
+  hence primed:"\<forall> r \<in> {0..\<tau>}. (D (\<lambda>\<tau>. \<theta> (x \<tau>) - \<nu> (x \<tau>)) \<mapsto> (\<lambda>\<tau>. \<tau> *\<^sub>R (\<theta>' (x r) - \<nu>' (x r))) 
+  at r within {0..\<tau>}) \<and> \<nu>' (x r) \<le> \<theta>' (x r)" 
+    using assms by (auto simp: has_vderiv_on_def has_vector_derivative_def)
+  hence "\<exists>r\<in>{0..\<tau>}. (\<theta> (x \<tau>) - \<nu> (x \<tau>)) - (\<theta> (x 0) - \<nu> (x 0)) = 
   (\<lambda>\<tau>. \<tau> *\<^sub>R (\<theta>' (x r) -  \<nu>' (x r))) (\<tau> - 0)" 
-    by(rule_tac closed_segment_mvt, auto simp: \<open>0 \<le> \<tau>\<close>)
-  then obtain r where "r \<in> {0--\<tau>}" 
+    by(rule_tac mvt_very_simple) (auto simp: tHyp)
+  then obtain r where "r \<in> {0..\<tau>}" 
     and "\<theta> (x \<tau>) - \<nu> (x \<tau>) = (\<tau> - 0) *\<^sub>R (\<theta>' (x r) -  \<nu>' (x r)) + (\<theta> (x 0) - \<nu> (x 0))" 
     by force 
   also have "... \<ge> 0" 
-    using tHyp(1) x_ivp(2) primed by (simp add: calculation(1))  
+    using tHyp(1) x_ivp(2) primed calculation(1) by auto 
   ultimately show "\<nu> (x \<tau>) \<le> \<theta> (x \<tau>)" 
     by simp
 qed
 
-lemma [ode_invariant_rules]:
+lemma [diff_invariant_rules]:
 fixes \<theta>::"'a::banach \<Rightarrow> real"
-assumes "\<forall> x. (D x = (\<lambda>\<tau>. f (x \<tau>)) on {0..t}) \<longrightarrow> (\<forall> \<tau> \<in> {0..t}. \<forall> r \<in> {0--\<tau>}. \<theta>' (x r) \<ge> \<nu>' (x r)
-\<and> (D (\<lambda>\<tau>. \<theta> (x \<tau>) - \<nu> (x \<tau>)) \<mapsto> (\<lambda>\<tau>. \<tau> *\<^sub>R (\<theta>' (x r) - \<nu>' (x r))) at r within {0--\<tau>}))"
+assumes "\<forall> x. (D x = (\<lambda>\<tau>. f (x \<tau>)) on {0..t}) \<longrightarrow> (\<forall>\<tau>\<in>{0..t}. \<theta>' (x \<tau>) \<ge> \<nu>' (x \<tau>) \<and> 
+  (D (\<lambda>\<tau>. \<theta> (x \<tau>) - \<nu> (x \<tau>)) = (\<lambda>r. \<theta>' (x r) - \<nu>' (x r)) on {0..\<tau>}))"
 shows "(\<lambda>s. \<nu> s < \<theta> s) is_diff_invariant_of f along {0..t}"
 proof(simp add: diff_invariant_def ivp_sols_def, clarsimp)
   fix x \<tau> assume tHyp:"0 \<le> \<tau>" "\<tau> \<le> t"
     and x_ivp:"D x = (\<lambda>\<tau>. f (x \<tau>)) on {0..t}" "\<nu> (x 0) < \<theta> (x 0)"
-  hence primed:"\<forall> r \<in> {0--\<tau>}. ((\<lambda>\<tau>. \<theta> (x \<tau>) - \<nu> (x \<tau>)) has_derivative 
-(\<lambda>\<tau>. \<tau> *\<^sub>R  (\<theta>' (x r) -  \<nu>' (x r)))) (at r within {0--\<tau>}) \<and> \<theta>' (x r) \<ge> \<nu>' (x r)" 
-    using assms by auto
-  hence "\<exists>r\<in>{0--\<tau>}. (\<theta> (x \<tau>) - \<nu> (x \<tau>)) - (\<theta> (x 0) - \<nu> (x 0)) = 
+  hence primed:"\<forall> r \<in> {0..\<tau>}. ((\<lambda>\<tau>. \<theta> (x \<tau>) - \<nu> (x \<tau>)) has_derivative 
+(\<lambda>\<tau>. \<tau> *\<^sub>R  (\<theta>' (x r) -  \<nu>' (x r)))) (at r within {0..\<tau>}) \<and> \<theta>' (x r) \<ge> \<nu>' (x r)" 
+    using assms by (auto simp: has_vderiv_on_def has_vector_derivative_def)
+  hence "\<exists>r\<in>{0..\<tau>}. (\<theta> (x \<tau>) - \<nu> (x \<tau>)) - (\<theta> (x 0) - \<nu> (x 0)) = 
   (\<lambda>\<tau>. \<tau> *\<^sub>R (\<theta>' (x r) -  \<nu>' (x r))) (\<tau> - 0)" 
-    by(rule_tac closed_segment_mvt, auto simp: \<open>0 \<le> \<tau>\<close>)
-  then obtain r where "r \<in> {0--\<tau>}" and 
+    by(rule_tac mvt_very_simple) (auto simp: tHyp)
+  then obtain r where "r \<in> {0..\<tau>}" and 
     "\<theta> (x \<tau>) - \<nu> (x \<tau>) = (\<tau> - 0) *\<^sub>R (\<theta>' (x r) -  \<nu>' (x r)) + (\<theta> (x 0) - \<nu> (x 0))" 
     by force 
   also have "... > 0" 
@@ -574,18 +549,16 @@ proof(simp add: diff_invariant_def ivp_sols_def, clarsimp)
     by simp
 qed
 
-lemma [ode_invariant_rules]:
-fixes \<theta>::"'a::banach \<Rightarrow> real"
-assumes "I1 is_diff_invariant_of f along {0..t}" 
-    and "I2 is_diff_invariant_of f along {0..t}"
-shows "(\<lambda>s. I1 s \<and> I2 s) is_diff_invariant_of f along {0..t}"
+lemma [diff_invariant_rules]:
+assumes "I\<^sub>1 is_diff_invariant_of f along {0..t}" 
+    and "I\<^sub>2 is_diff_invariant_of f along {0..t}"
+shows "(\<lambda>s. I\<^sub>1 s \<and> I\<^sub>2 s) is_diff_invariant_of f along {0..t}"
   using assms unfolding diff_invariant_def by auto
 
-lemma [ode_invariant_rules]:
-fixes \<theta>::"'a::banach \<Rightarrow> real"
-assumes "I1 is_diff_invariant_of f along {0..t}" 
-    and "I2 is_diff_invariant_of f along {0..t}"
-shows "(\<lambda>s. I1 s \<or> I2 s) is_diff_invariant_of f along {0..t}"
+lemma [diff_invariant_rules]:
+assumes "I\<^sub>1 is_diff_invariant_of f along {0..t}" 
+    and "I\<^sub>2 is_diff_invariant_of f along {0..t}"
+shows "(\<lambda>s. I\<^sub>1 s \<or> I\<^sub>2 s) is_diff_invariant_of f along {0..t}"
   using assms unfolding diff_invariant_def by auto
 
 end
