HybridVerifVecs/rels/cat2rel.thy
@@ -7,11 +7,13 @@ begin
 
 chapter\<open> Hybrid System Verification with relations \<close>
 
+
 \<comment> \<open>We start by deleting some conflicting notation.\<close>
 no_notation Archimedean_Field.ceiling ("\<lceil>_\<rceil>")
         and Archimedean_Field.floor_ceiling_class.floor ("\<lfloor>_\<rfloor>")
         and Range_Semiring.antirange_semiring_class.ars_r ("r")
         and Relation.Domain ("r2s")
+        and VC_KAD.gets ("_ ::= _" [70, 65] 61)
 
 section\<open> Verification of regular programs \<close>
 
@@ -19,10 +21,7 @@ text\<open> Below we explore the behavior of the forward box operator from the a
 with the lifting ($\lceil-\rceil$*) operator from predicates to relations @{thm p2r_def[no_vars]} 
 and its dropping counterpart @{thm r2p_def[no_vars]}. \<close>
 
-lemma p2r_IdD:"\<lceil>P\<rceil> = Id \<Longrightarrow> P s"
-  by (metis (full_types) UNIV_I impl_prop p2r_subid top_empty_eq)
-
-lemma wp_rel:"wp R \<lceil>P\<rceil> = \<lceil>\<lambda> x. \<forall> y. (x,y) \<in> R \<longrightarrow> P y\<rceil>"
+lemma wp_rel: "wp R \<lceil>P\<rceil> = \<lceil>\<lambda> x. \<forall> y. (x,y) \<in> R \<longrightarrow> P y\<rceil>"
 proof-
   have "\<lfloor>wp R \<lceil>P\<rceil>\<rfloor> = \<lfloor>\<lceil>\<lambda> x. \<forall> y. (x,y) \<in> R \<longrightarrow> P y\<rceil>\<rfloor>" 
     by (simp add: wp_trafo pointfree_idE)
@@ -30,31 +29,22 @@ proof-
     by (metis (no_types, lifting) wp_simp d_p2r pointfree_idE prp) 
 qed
 
-corollary wp_relD:"(x,x) \<in> wp R \<lceil>P\<rceil> \<Longrightarrow> \<forall> y. (x,y) \<in> R \<longrightarrow> P y"
-proof-
-  assume "(x,x) \<in> wp R \<lceil>P\<rceil>"
-  hence "(x,x) \<in> \<lceil>\<lambda> x. \<forall> y. (x,y) \<in> R \<longrightarrow> P y\<rceil>" using wp_rel by auto
-  thus "\<forall> y. (x,y) \<in> R \<longrightarrow> P y" by (simp add: p2r_def)
-qed
-
-lemma p2r_r2p_wp_sym:"wp R P = \<lceil>\<lfloor>wp R P\<rfloor>\<rceil>"
-  using d_p2r wp_simp by blast
-
-lemma p2r_r2p_wp:"\<lceil>\<lfloor>wp R P\<rfloor>\<rceil> = wp R P"
-  by(rule sym, subst p2r_r2p_wp_sym, simp)
+lemma p2r_r2p_wp: "\<lceil>\<lfloor>wp R P\<rfloor>\<rceil> = wp R P"
+  apply(subst d_p2r[symmetric])
+  using wp_simp[symmetric, of R P] by blast
 
 text\<open> Next, we introduce assignments and compute their @{text "wp"}. \<close>
 
-abbreviation vec_upd :: "('a^'b) \<Rightarrow> 'b \<Rightarrow> 'a \<Rightarrow> 'a^'b" ("_(2[_ :== _])" [70, 65] 61) where 
-"x[i :== a] \<equiv> (\<chi> j. (if j = i then a else (x $ j)))"
+abbreviation vec_upd :: "('a^'b) \<Rightarrow> 'b \<Rightarrow> 'a \<Rightarrow> 'a^'b"
+  where "vec_upd x i a \<equiv> vec_lambda ((vec_nth x)(i := a))"
 
-abbreviation assign :: "'b \<Rightarrow> ('a^'b \<Rightarrow> 'a) \<Rightarrow> ('a^'b) rel" ("(2[_ ::== _])" [70, 65] 61) where 
-"[x ::== expr]\<equiv> {(s, s[x :== expr s])| s. True}" 
+abbreviation assign :: "'b \<Rightarrow> ('a^'b \<Rightarrow> 'a) \<Rightarrow> ('a^'b) rel" ("(2_ ::= _)" [70, 65] 61) 
+  where "(x ::= e) \<equiv> {(s, vec_upd s x (e s))| s. True}" 
 
-lemma wp_assign [simp]: "wp ([x ::== expr]) \<lceil>Q\<rceil> = \<lceil>\<lambda>s. Q (s[x :== expr s])\<rceil>"
+lemma wp_assign [simp]: "wp (x ::= e) \<lceil>Q\<rceil> = \<lceil>\<lambda>s. Q (vec_upd s x (e s))\<rceil>"
   by(auto simp: rel_antidomain_kleene_algebra.fbox_def rel_ad_def p2r_def)
 
-lemma wp_assign_var [simp]: "\<lfloor>wp ([x ::== expr]) \<lceil>Q\<rceil>\<rfloor> = (\<lambda>s. Q (s[x :== expr s]))"
+lemma wp_assign_var [simp]: "\<lfloor>wp (x ::= e) \<lceil>Q\<rceil>\<rfloor> = (\<lambda>s. Q (vec_upd s x (e s)))"
   by(subst wp_assign, simp add: pointfree_idE)
 
 text\<open> The @{text "wp"} of the composition was already obtained in KAD.Antidomain\_Semiring:
@@ -66,29 +56,34 @@ and its @{text "wp"}: @{thm fbox_cond[no_vars]}. \<close>
 text\<open> Finally, we add a wp-rule for a simple finite iteration. \<close>
 
 lemma (in antidomain_kleene_algebra) fbox_starI: 
-assumes "d p \<le> d i" and "d i \<le> |x] i" and "d i \<le> d q"
-shows "d p \<le> |x\<^sup>\<star>] q"
+  assumes "d p \<le> d i" and "d i \<le> |x] i" and "d i \<le> d q"
+  shows "d p \<le> |x\<^sup>\<star>] q"
 proof-
-from \<open>d i \<le> |x] i\<close> have "d i \<le> |x] (d i)"
-  using local.fbox_simp by auto 
-hence "|1] p \<le> |x\<^sup>\<star>] i" using \<open>d p \<le> d i\<close> by (metis (no_types) 
-  local.dual_order.trans local.fbox_one local.fbox_simp local.fbox_star_induct_var)
-thus ?thesis using \<open>d i \<le> d q\<close> by (metis (full_types)
-  local.fbox_mult local.fbox_one local.fbox_seq_var local.fbox_simp)
+  have "d i \<le> |x] (d i)"
+    using \<open>d i \<le> |x] i\<close> local.fbox_simp by auto
+  hence "|1] p \<le> |x\<^sup>\<star>] i" 
+    using \<open>d p \<le> d i\<close> by (metis (no_types) dual_order.trans 
+        fbox_one fbox_simp fbox_star_induct_var)
+  thus ?thesis 
+    using \<open>d i \<le> d q\<close> by (metis (full_types) fbox_mult 
+        fbox_one fbox_seq_var fbox_simp)
 qed
 
 lemma rel_ad_mka_starI:
-assumes "P \<subseteq> I" and "I \<subseteq> wp R I" and "I \<subseteq> Q"
-shows "P \<subseteq> wp (R\<^sup>*) Q"
+  assumes "P \<subseteq> I" and "I \<subseteq> wp R I" and "I \<subseteq> Q"
+  shows "P \<subseteq> wp (R\<^sup>*) Q"
 proof-
   have "wp R I \<subseteq> Id"
     by (simp add: rel_antidomain_kleene_algebra.a_subid rel_antidomain_kleene_algebra.fbox_def)
-  hence "P \<subseteq> Id" using assms(1,2) by blast
-  from this have "rdom P = P" by (metis d_p2r p2r_surj)
+  hence "P \<subseteq> Id" 
+    using assms(1,2) by blast
+  hence "rdom P = P" 
+    by (metis d_p2r p2r_surj)
   also have "rdom P \<subseteq> wp (R\<^sup>*) Q"
-    by (metis \<open>wp R I \<subseteq> Id\<close> assms d_p2r p2r_surj 
-        rel_antidomain_kleene_algebra.dka.dom_iso rel_antidomain_kleene_algebra.fbox_starI)
-  ultimately show ?thesis by blast
+    by (metis \<open>wp R I \<subseteq> Id\<close> assms d_p2r p2r_surj rel_antidomain_kleene_algebra.dka.dom_iso 
+        rel_antidomain_kleene_algebra.fbox_starI)
+  ultimately show ?thesis 
+    by blast
 qed
 
 
@@ -112,25 +107,18 @@ lemma ivp_solsD:
     and "x t\<^sub>0 = s" and "t\<^sub>0 \<in> T"
   using assms unfolding ivp_sols_def by auto
 
-lemma "(t::real) \<in> {0--t}"
-  by (rule ends_in_segment(2))
-
-lemma "(t::real) \<in> {0..t}"
-  apply auto
-  oops
-
-definition "g_orbital f T t\<^sub>0 G s = \<Union> {{x t|t. t \<in> T \<and> G \<rhd> x {t\<^sub>0--t} }|x. x \<in> ivp_sols f T t\<^sub>0 s}"
+definition "g_orbital f T t\<^sub>0 G s = \<Union> {{x t|t. t \<in> T \<and> G \<rhd> x {t\<^sub>0..t} }|x. x \<in> ivp_sols f T t\<^sub>0 s}"
 
 lemma g_orbital_eq: "g_orbital f T t\<^sub>0 G s = 
-  {x t |t x. t \<in> T \<and> (D x = (f \<circ> x) on T) \<and> x t\<^sub>0 = s \<and> t\<^sub>0 \<in> T \<and> G \<rhd> x {t\<^sub>0--t}}"
+  {x t |t x. t \<in> T \<and> (D x = (f \<circ> x) on T) \<and> x t\<^sub>0 = s \<and> t\<^sub>0 \<in> T \<and> G \<rhd> x {t\<^sub>0..t}}"
   unfolding g_orbital_def ivp_sols_def by auto
 
-lemma "g_orbital f T t\<^sub>0 G s = (\<Union> x \<in> ivp_sols f T t\<^sub>0 s. {x t|t. t \<in> T \<and> G \<rhd> x {t\<^sub>0--t}})"
+lemma "g_orbital f T t\<^sub>0 G s = (\<Union> x \<in> ivp_sols f T t\<^sub>0 s. {x t|t. t \<in> T \<and> G \<rhd> x {t\<^sub>0..t}})"
   unfolding g_orbital_def ivp_sols_def by auto
 
 lemma g_orbitalI:
   assumes "D x = (f \<circ> x) on T" "x t\<^sub>0 = s"
-    and "t\<^sub>0 \<in> T" "t \<in> T" and "G \<rhd> x {t\<^sub>0--t}"
+    and "t\<^sub>0 \<in> T" "t \<in> T" and "G \<rhd> x {t\<^sub>0..t}"
   shows "x t \<in> g_orbital f T t\<^sub>0 G s"
   using assms unfolding g_orbital_def ivp_sols_def by blast
 
@@ -138,7 +126,7 @@ lemma g_orbitalD:
   assumes "s' \<in> g_orbital f T t\<^sub>0 G s"
   obtains x and t where "x \<in> ivp_sols f T t\<^sub>0 s" 
   and "D x = (f \<circ> x) on T" "x t\<^sub>0 = s"
-  and "x t = s'" and "t\<^sub>0 \<in> T" "t \<in> T" and "G \<rhd> x {t\<^sub>0--t}"
+  and "x t = s'" and "t\<^sub>0 \<in> T" "t \<in> T" and "G \<rhd> x {t\<^sub>0..t}"
   using assms unfolding g_orbital_def ivp_sols_def by blast
 
 abbreviation g_evol :: "(('a::banach) \<Rightarrow> 'a) \<Rightarrow> real set \<Rightarrow>'a pred \<Rightarrow> 'a rel" ("(1[x\<acute>=_]_ & _)") 
@@ -159,24 +147,26 @@ lemma orbit_eq[simp]: "orbit s = {\<phi> t s| t. t \<in> T}"
   by(auto intro: usolves_ivp intro!: ivp simp: init_time)
 
 lemma g_orbital_collapses: 
-  shows "g_orbital f T 0 G s = {\<phi> t s | t. t \<in> T \<and> G \<rhd> (\<lambda>r. \<phi> r s) {0--t}}" (is "_ = ?gorbit")
+  shows "g_orbital f T 0 G s = {\<phi> t s | t. t \<in> T \<and> G \<rhd> (\<lambda>r. \<phi> r s) {0..t}}" (is "_ = ?gorbit")
 proof(rule subset_antisym, simp_all only: subset_eq)
   {fix s' assume "s' \<in> g_orbital f T 0 G s"
-    then obtain x and t where x_ivp:"D x = (f \<circ> x) on T" 
-      "x 0 = s" and "x t = s'" and "t \<in> T" and guard:"G \<rhd> x {0--t}"
-      unfolding g_orbital_eq by blast
-    hence obs:"\<forall>\<tau>\<in>{0--t}. x \<tau> = \<phi> \<tau> s"
-      using usolves_ivp[of x s] closed_segment_subset_domainI init_time comp_def
-      by (metis (mono_tags, lifting) has_vderiv_eq)
-    hence "G \<rhd> (\<lambda>r. \<phi> r s) {0--t}"
+    then obtain x and t where x_ivp:"D x = (\<lambda>t. f (x t)) on T" 
+      "x 0 = s" and "x t = s'" and "t \<in> T" and guard:"G \<rhd> x {0..t}"
+      unfolding g_orbital_eq by auto
+    hence obs:"\<forall>\<tau>\<in>{0..t}. x \<tau> = \<phi> \<tau> s"
+      using usolves_ivp[OF x_ivp]
+      by (meson atLeastAtMost_iff init_time interval mem_is_interval_1_I) 
+    hence "G \<rhd> (\<lambda>r. \<phi> r s) {0..t}"
       using guard by simp
-    hence "s' \<in> ?gorbit"
-      using \<open>x t = s'\<close> \<open>t \<in> T\<close> obs by blast}
+    also have "\<phi> t s = x t"
+      using usolves_ivp x_ivp \<open>t \<in> T\<close> by simp
+    ultimately have "s' \<in> ?gorbit"
+      using \<open>x t = s'\<close> \<open>t \<in> T\<close> by auto}
   thus "\<forall>s'\<in>g_orbital f T 0 G s. s' \<in> ?gorbit"
     by blast
 next
   {fix s' assume "s' \<in> ?gorbit"
-    then obtain t where "G \<rhd> (\<lambda>r. \<phi> r s) {0--t}" and "t \<in> T" and "\<phi> t s = s'"
+    then obtain t where "G \<rhd> (\<lambda>r. \<phi> r s) {0..t}" and "t \<in> T" and "\<phi> t s = s'"
       by blast
     hence "s' \<in> g_orbital f T 0 G s"
       by(auto intro: g_orbitalI simp: ivp init_time)}
@@ -185,19 +175,21 @@ next
 qed
 
 lemma g_evol_collapses:
-  shows "([x\<acute>=f]T & G) = {(s, \<phi> t s) | t s. t \<in> T \<and> G \<rhd> (\<lambda>r. \<phi> r s) {0--t}}"
+  shows "([x\<acute>=f]T & G) = {(s, \<phi> t s) | t s. t \<in> T \<and> G \<rhd> (\<lambda>r. \<phi> r s) {0..t}}"
   unfolding g_orbital_collapses by auto
 
 lemma wp_orbit: "wp ({(s,s') | s s'. s' \<in> orbit s}) \<lceil>Q\<rceil> = \<lceil>\<lambda> s. \<forall> t \<in> T. Q (\<phi> t s)\<rceil>"
   unfolding orbit_eq wp_rel by auto
 
-lemma wp_g_orbit: "wp ([x\<acute>=f]T & G) \<lceil>Q\<rceil> = \<lceil>\<lambda> s. \<forall>t\<in>T. (G \<rhd> (\<lambda>r. \<phi> r s) {0--t}) \<longrightarrow> Q (\<phi> t s)\<rceil>"
+lemma wp_g_orbit: "wp ([x\<acute>=f]T & G) \<lceil>Q\<rceil> = \<lceil>\<lambda> s. \<forall>t\<in>T. (G \<rhd> (\<lambda>r. \<phi> r s) {0..t}) \<longrightarrow> Q (\<phi> t s)\<rceil>"
   unfolding g_evol_collapses wp_rel by auto
 
 end
 
-lemma (in global_flow) ivp_sols_collapse[simp]: "ivp_sols f UNIV 0 s = {(\<lambda>t. \<phi> t s)}"
-  by(auto intro: usolves_ivp simp: ivp_sols_def ivp)
+lemma (in local_flow) ivp_sols_collapse: "ivp_sols f T 0 s = {(\<lambda>t. \<phi> t s)}"
+  apply(auto simp: ivp_sols_def ivp init_time fun_eq_iff)
+  apply(rule unique_solution, simp_all add: ivp)
+  oops
 
 text\<open> The previous theorem allows us to compute wlps for known systems of ODEs. We can also implement
 a version of it as an inference rule. A simple computation of a wlp is shown immmediately after.\<close>
@@ -206,11 +198,10 @@ lemma dSolution:
   assumes "local_flow f T L \<phi>"
     and "\<forall>s. P s \<longrightarrow> (\<forall> t \<in> T. (G \<rhd> (\<lambda>r. \<phi> r s) {0..t}) \<longrightarrow> Q (\<phi> t s))"
   shows "\<lceil>P\<rceil> \<le> wp ([x\<acute>=f]T & G) \<lceil>Q\<rceil>"
-  using assms apply(subst local_flow.wp_g_orbit, auto)
-  by (simp add: Starlike.closed_segment_eq_real_ivl)
+  using assms by(subst local_flow.wp_g_orbit, auto)
 
 lemma line_DS: "0 \<le> t \<Longrightarrow> wp ([x\<acute>=\<lambda>s. c]{0..t} & G) \<lceil>Q\<rceil> = 
-    \<lceil>\<lambda> x. \<forall> \<tau> \<in> {0..t}. (G \<rhd> (\<lambda>r. x + r *\<^sub>R c) {0..\<tau>}) \<longrightarrow> Q (x + \<tau> *\<^sub>R c)\<rceil>"
+  \<lceil>\<lambda> x. \<forall>\<tau>\<in>{0..t}. (G \<rhd> (\<lambda>t. x + t *\<^sub>R c) {0..\<tau>}) \<longrightarrow> Q (x + \<tau> *\<^sub>R c)\<rceil>"
   apply(subst local_flow.wp_g_orbit[of "\<lambda>s. c" _ "1/(t + 1)" "(\<lambda> t x. x + t *\<^sub>R c)"])
   by(auto simp: line_is_local_flow closed_segment_eq_real_ivl)
   
@@ -224,23 +215,22 @@ Then we prove the inference rules which are used in verification proofs.\<close>
 
 subsubsection\<open> Differential Weakening \<close>
 
-lemma DW: "wp ([x\<acute>=f]T & G) \<lceil>Q\<rceil> = wp ([x\<acute>=f]T & G) \<lceil>\<lambda> s. G s \<longrightarrow> Q s\<rceil>"
-  apply(subst wp_rel)+
-  by(auto simp: g_orbital_eq)
+lemma DW: "wp ([x\<acute>=f]{0..t} & G) \<lceil>Q\<rceil> = wp ([x\<acute>=f]{0..t} & G) \<lceil>\<lambda> s. G s \<longrightarrow> Q s\<rceil>"
+  by (auto intro: g_orbitalD simp: wp_rel)
 
 lemma dWeakening: 
   assumes "\<lceil>G\<rceil> \<le> \<lceil>Q\<rceil>"
-  shows "\<lceil>P\<rceil> \<le> wp ([x\<acute>=f]T & G) \<lceil>Q\<rceil>"
+  shows "\<lceil>P\<rceil> \<le> wp ([x\<acute>=f]{0..t} & G) \<lceil>Q\<rceil>"
   using assms apply(subst wp_rel)
-  by(auto simp: g_orbital_eq)
+  by(auto simp: g_evol_def)
 
 subsubsection\<open> Differential Cut \<close>
 
 lemma wp_g_orbit_IdD:
-  assumes "wp ([x\<acute>=f]T & G) \<lceil>C\<rceil> = Id" and "\<forall> r\<in>{0--t}. (s, x r) \<in> ([x\<acute>=f]T & G)"
-  shows "\<forall>r\<in>{0--t}. C (x r)"
+  assumes "wp ([x\<acute>=f]T & G) \<lceil>C\<rceil> = Id" and "\<forall> r\<in>{0..t}. (s, x r) \<in> ([x\<acute>=f]T & G)"
+  shows "\<forall>r\<in>{0..t}. C (x r)"
 proof
-  fix r assume "r \<in> {0--t}"
+  fix r assume "r \<in> {0..t}"
   then have "x r \<in> g_orbital f T 0 G s" 
     using assms(2) by blast
   also have "\<forall>y. y \<in> (g_orbital f T 0 G s) \<longrightarrow> C y" 
@@ -254,17 +244,17 @@ theorem DC:
 proof(rule_tac f="\<lambda> x. wp x \<lceil>Q\<rceil>" in HOL.arg_cong, rule subset_antisym, safe)
   {fix s and s' assume "s' \<in> g_orbital f T 0 G s"
     then obtain t::real and x where x_ivp: "D x = (f \<circ> x) on T" "x 0 = s"
-      and guard_x:"G \<rhd> x {0--t}" and "s' = x t" and "0 \<in> T" "t \<in> T"
+      and guard_x:"G \<rhd> x {0..t}" and "s' = x t" and "0 \<in> T" "t \<in> T"
       using g_orbitalD[of s' "f" T 0 G s] by (metis (full_types))
-    from guard_x have "\<forall>r\<in>{0--t}.\<forall> \<tau>\<in>{0--r}. G (x \<tau>)"
-      by (metis contra_subsetD ends_in_segment(1) subset_segment(1))
-    also have "\<forall>\<tau>\<in>{0--t}. \<tau> \<in> T"
-      using interval.closed_segment_subset_domain[OF assms(1) \<open>0 \<in> T\<close> \<open>t \<in> T\<close>] by blast
-    ultimately have "\<forall>\<tau>\<in>{0--t}. x \<tau> \<in> g_orbital f T 0 G s"
+    from guard_x have "\<forall>r\<in>{0..t}.\<forall>\<tau>\<in>{0..r}. G (x \<tau>)"
+      by auto
+    also have "\<forall>\<tau>\<in>{0..t}. \<tau> \<in> T"
+      by (meson \<open>0 \<in> T\<close> \<open>t \<in> T\<close> assms(1) atLeastAtMost_iff interval.interval mem_is_interval_1_I)
+    ultimately have "\<forall>\<tau>\<in>{0..t}. x \<tau> \<in> g_orbital f T 0 G s"
       using g_orbitalI[OF x_ivp \<open>0 \<in> T\<close>] by blast
-    hence "\<forall>\<tau>\<in>{0--t}. (s, x \<tau>) \<in> [x\<acute>=f]T & G"
+    hence "\<forall>\<tau>\<in>{0..t}. (s, x \<tau>) \<in> [x\<acute>=f]T & G"
       unfolding wp_rel by(auto simp: p2r_def)
-    hence "C \<rhd> x {0--t}" 
+    hence "C \<rhd> x {0..t}" 
       using wp_g_orbit_IdD[OF assms(2)] by blast
     hence "s' \<in> g_orbital f T 0 (\<lambda>s. G s \<and> C s) s"
       using g_orbitalI[OF x_ivp \<open>0 \<in> T\<close> \<open>t \<in> T\<close>] guard_x \<open>s' = x t\<close> by fastforce}
@@ -279,18 +269,19 @@ theorem dCut:
     and wp_Q:"\<lceil>P\<rceil> \<subseteq> wp ([x\<acute>=f]{0..t} & (\<lambda> s. G s \<and> C s)) \<lceil>Q\<rceil>"
   shows "\<lceil>P\<rceil> \<subseteq> wp ([x\<acute>=f]{0..t} & G) \<lceil>Q\<rceil>"
 proof(subst wp_rel, simp add: g_orbital_eq p2r_def, clarsimp)
-  fix \<tau>::real and x::"real \<Rightarrow> 'a" assume "P (x 0)" and "0 \<le> \<tau>" and "\<tau> \<le> t"
-    and x_solves:"D x = (\<lambda>t. f (x t)) on {0..t}" and guard_x:"(\<forall> r \<in> {0--\<tau>}. G (x r))"
-  hence "\<forall>r\<in>{0--\<tau>}.\<forall>\<tau>\<in>{0--r}. G (x \<tau>)"
-    using closed_segment_closed_segment_subset by blast
-  hence "\<forall>r\<in>{0--\<tau>}. x r \<in> g_orbital f {0..t} 0 G (x 0)"
-    using g_orbitalI x_solves \<open>0 \<le> \<tau>\<close> \<open>\<tau> \<le> t\<close> closed_segment_eq_real_ivl by fastforce 
-  hence "\<forall>r\<in>{0--\<tau>}. C (x r)" 
+  fix \<tau>::real and x::"real \<Rightarrow> 'a" 
+  assume guard_x:"(\<forall> r \<in> {0..\<tau>}. G (x r))" and "0 \<le> \<tau>" and "\<tau> \<le> t"
+    and x_solves:"D x = (\<lambda>t. f (x t)) on {0..t}" and "P (x 0)"
+  hence "\<forall>r\<in>{0..\<tau>}.\<forall>\<tau>\<in>{0..r}. G (x \<tau>)"
+    by auto
+  hence "\<forall>r\<in>{0..\<tau>}. x r \<in> g_orbital f {0..t} 0 G (x 0)"
+    using g_orbitalI x_solves \<open>0 \<le> \<tau>\<close> \<open>\<tau> \<le> t\<close> by fastforce 
+  hence "\<forall>r\<in>{0..\<tau>}. C (x r)" 
     using wp_C \<open>P (x 0)\<close> by(subst (asm) wp_rel, auto)
   hence "x \<tau> \<in> g_orbital f {0..t} 0 (\<lambda>s. G s \<and> C s) (x 0)"
     using g_orbitalI x_solves guard_x \<open>0 \<le> \<tau>\<close> \<open>\<tau> \<le> t\<close> by fastforce
   from this \<open>P (x 0)\<close> and wp_Q show "Q (x \<tau>)"
-    by(subst (asm) wp_rel, auto simp: closed_segment_eq_real_ivl)
+    by(subst (asm) wp_rel, auto)
 qed
 
 subsubsection\<open> Differential Invariant \<close>
@@ -304,7 +295,7 @@ lemma DI_sufficiency:
   apply(erule exE, erule impE)
   by(rule_tac x="0" in exI, rule_tac x=x in exI, auto)
 
-lemma (in local_flow) DI_necessity: (* Not true... check Bohrer formalisation *)
+lemma (in local_flow) DI_necessity:
   shows "wp \<lceil>G\<rceil> \<lceil>Q\<rceil> \<le> wp ([x\<acute>=f]T & G) \<lceil>Q\<rceil>"
   unfolding wp_g_orbit apply(subst wp_rel, simp add: p2r_def, clarsimp)
    apply(erule_tac x="0" in ballE)
@@ -312,8 +303,8 @@ lemma (in local_flow) DI_necessity: (* Not true... check Bohrer formalisation *)
   oops
 
 definition diff_invariant :: "'a pred \<Rightarrow> (('a::real_normed_vector) \<Rightarrow> 'a) \<Rightarrow> real set \<Rightarrow> bool" 
-("(_)/ is'_diff'_invariant'_of (_)/ along (_)" [70,65]61) 
-where "I is_diff_invariant_of f along T \<equiv> 
+  ("(_)/ is'_diff'_invariant'_of (_)/ along (_)" [70,65]61) 
+  where "I is_diff_invariant_of f along T \<equiv> 
   (\<forall>s. I s \<longrightarrow> (\<forall> x. x \<in> ivp_sols f T 0 s \<longrightarrow> (\<forall> t \<in> T. I (x t))))"
 
 lemma invariant_to_set:
@@ -325,7 +316,6 @@ lemma invariant_to_set:
   apply(drule mp, simp_all add: subset_eq)
   apply(erule_tac x="xa t" in allE)
   by(drule mp, auto)
-
 
 lemma dInvariant:
   assumes "I is_diff_invariant_of f along T"
@@ -345,61 +335,61 @@ lemma dI:
 
 text\<open> Finally, we obtain some conditions to prove specific instances of differential invariants. \<close>
 
-named_theorems ode_invariant_rules "compilation of rules for differential invariants."
+named_theorems diff_invariant_rules "compilation of rules for differential invariants."
 
-lemma [ode_invariant_rules]:
-fixes \<theta>::"'a::banach \<Rightarrow> real"
-assumes "\<forall> x. (D x = (\<lambda>\<tau>. f (x \<tau>)) on {0..t}) \<longrightarrow> (\<forall> \<tau> \<in> {0..t}. \<forall> r \<in> {0--\<tau>}. 
-  ((\<lambda>\<tau>. \<theta> (x \<tau>) - \<nu> (x \<tau>) ) has_derivative (\<lambda>\<tau>.  \<tau> *\<^sub>R 0)) (at r within {0--\<tau>}))"
-shows "(\<lambda>s. \<theta> s = \<nu> s) is_diff_invariant_of f along {0..t}"
+lemma [diff_invariant_rules]:
+  fixes \<theta>::"'a::banach \<Rightarrow> real"
+  assumes "\<forall>x. (D x = (\<lambda>\<tau>. f (x \<tau>)) on {0..t}) \<longrightarrow> 
+  (\<forall>\<tau>\<in>{0..t}. (D (\<lambda>\<tau>. \<theta> (x \<tau>) - \<nu> (x \<tau>)) = ((*\<^sub>R) 0) on {0..\<tau>}))"
+  shows "(\<lambda>s. \<theta> s = \<nu> s) is_diff_invariant_of f along {0..t}"
 proof(simp add: diff_invariant_def ivp_sols_def, clarsimp)
   fix x \<tau> assume tHyp:"0 \<le> \<tau>" "\<tau> \<le> t" 
     and x_ivp:"D x = (\<lambda>\<tau>. f (x \<tau>)) on {0..t}" "\<theta> (x 0) = \<nu> (x 0)" 
-  hence "\<forall> r \<in> {0--\<tau>}. D (\<lambda>\<tau>. \<theta> (x \<tau>) - \<nu> (x \<tau>)) \<mapsto> (\<lambda>\<tau>. \<tau> *\<^sub>R 0) at r within {0--\<tau>}" 
-    using assms by auto
-  hence "\<exists>r\<in>{0--\<tau>}. (\<theta> (x \<tau>) - \<nu> (x \<tau>)) - (\<theta> (x 0) - \<nu> (x 0)) = (\<lambda>\<tau>. \<tau> *\<^sub>R 0) (\<tau> - 0)" 
-    by(rule_tac closed_segment_mvt, auto simp: tHyp) 
+  hence "\<forall> t \<in> {0..\<tau>}. D (\<lambda>\<tau>. \<theta> (x \<tau>) - \<nu> (x \<tau>)) \<mapsto> (\<lambda>\<tau>. \<tau> *\<^sub>R 0) at t within {0..\<tau>}" 
+    using assms by (auto simp: has_vderiv_on_def has_vector_derivative_def)
+  hence "\<exists>t\<in>{0..\<tau>}. \<theta> (x \<tau>) - \<nu> (x \<tau>) - (\<theta> (x 0) - \<nu> (x 0)) = (\<tau> - 0) \<cdot> 0" 
+    by(rule_tac mvt_very_simple) (auto simp: tHyp)
   thus "\<theta> (x \<tau>) = \<nu> (x \<tau>)" by (simp add: x_ivp(2))
 qed
 
-lemma [ode_invariant_rules]:
-fixes \<theta>::"'a::banach \<Rightarrow> real"
-assumes "\<forall> x. (D x = (\<lambda>\<tau>. f (x \<tau>)) on {0..t}) \<longrightarrow> (\<forall> \<tau> \<in> {0..t}. \<forall> r \<in> {0--\<tau>}. \<theta>' (x r) \<ge> \<nu>' (x r)
-\<and> (D (\<lambda>\<tau>. \<theta> (x \<tau>) - \<nu> (x \<tau>)) \<mapsto> (\<lambda>\<tau>. \<tau> *\<^sub>R (\<theta>' (x r) - \<nu>' (x r))) at r within {0--\<tau>}))"
-shows "(\<lambda>s. \<nu> s \<le> \<theta> s) is_diff_invariant_of f along {0..t}"
+lemma [diff_invariant_rules]:
+  fixes \<theta>::"'a::banach \<Rightarrow> real"
+  assumes "\<forall> x. (D x = (\<lambda>\<tau>. f (x \<tau>)) on {0..t}) \<longrightarrow> (\<forall>\<tau>\<in>{0..t}. \<theta>' (x \<tau>) \<ge> \<nu>' (x \<tau>) \<and> 
+  (D (\<lambda>\<tau>. \<theta> (x \<tau>) - \<nu> (x \<tau>)) = (\<lambda>r. \<theta>' (x r) - \<nu>' (x r)) on {0..\<tau>}))"
+  shows "(\<lambda>s. \<nu> s \<le> \<theta> s) is_diff_invariant_of f along {0..t}"
 proof(simp add: diff_invariant_def ivp_sols_def, clarsimp)
   fix x \<tau> assume tHyp:"0 \<le> \<tau>" "\<tau> \<le> t" 
     and x_ivp:"D x = (\<lambda>\<tau>. f (x \<tau>)) on {0..t}" "\<nu> (x 0) \<le> \<theta> (x 0)"
-  hence primed:"\<forall> r \<in> {0--\<tau>}. (D (\<lambda>\<tau>. \<theta> (x \<tau>) - \<nu> (x \<tau>)) \<mapsto> (\<lambda>\<tau>. \<tau> *\<^sub>R (\<theta>' (x r) - \<nu>' (x r))) 
-  at r within {0--\<tau>}) \<and> \<nu>' (x r) \<le> \<theta>' (x r)" 
-    using assms by auto
-  hence "\<exists>r\<in>{0--\<tau>}. (\<theta> (x \<tau>) - \<nu> (x \<tau>)) - (\<theta> (x 0) - \<nu> (x 0)) = 
+  hence primed:"\<forall> r \<in> {0..\<tau>}. (D (\<lambda>\<tau>. \<theta> (x \<tau>) - \<nu> (x \<tau>)) \<mapsto> (\<lambda>\<tau>. \<tau> *\<^sub>R (\<theta>' (x r) - \<nu>' (x r))) 
+  at r within {0..\<tau>}) \<and> \<nu>' (x r) \<le> \<theta>' (x r)" 
+    using assms by (auto simp: has_vderiv_on_def has_vector_derivative_def)
+  hence "\<exists>r\<in>{0..\<tau>}. (\<theta> (x \<tau>) - \<nu> (x \<tau>)) - (\<theta> (x 0) - \<nu> (x 0)) = 
   (\<lambda>\<tau>. \<tau> *\<^sub>R (\<theta>' (x r) -  \<nu>' (x r))) (\<tau> - 0)" 
-    by(rule_tac closed_segment_mvt, auto simp: \<open>0 \<le> \<tau>\<close>)
-  then obtain r where "r \<in> {0--\<tau>}" 
+    by(rule_tac mvt_very_simple) (auto simp: tHyp)
+  then obtain r where "r \<in> {0..\<tau>}" 
     and "\<theta> (x \<tau>) - \<nu> (x \<tau>) = (\<tau> - 0) *\<^sub>R (\<theta>' (x r) -  \<nu>' (x r)) + (\<theta> (x 0) - \<nu> (x 0))" 
     by force 
   also have "... \<ge> 0" 
-    using tHyp(1) x_ivp(2) primed by (simp add: calculation(1))  
+    using tHyp(1) x_ivp(2) primed calculation(1) by auto 
   ultimately show "\<nu> (x \<tau>) \<le> \<theta> (x \<tau>)" 
     by simp
 qed
 
-lemma [ode_invariant_rules]:
+lemma [diff_invariant_rules]:
 fixes \<theta>::"'a::banach \<Rightarrow> real"
-assumes "\<forall> x. (D x = (\<lambda>\<tau>. f (x \<tau>)) on {0..t}) \<longrightarrow> (\<forall> \<tau> \<in> {0..t}. \<forall> r \<in> {0--\<tau>}. \<theta>' (x r) \<ge> \<nu>' (x r)
-\<and> (D (\<lambda>\<tau>. \<theta> (x \<tau>) - \<nu> (x \<tau>)) \<mapsto> (\<lambda>\<tau>. \<tau> *\<^sub>R (\<theta>' (x r) - \<nu>' (x r))) at r within {0--\<tau>}))"
+assumes "\<forall> x. (D x = (\<lambda>\<tau>. f (x \<tau>)) on {0..t}) \<longrightarrow> (\<forall>\<tau>\<in>{0..t}. \<theta>' (x \<tau>) \<ge> \<nu>' (x \<tau>) \<and> 
+  (D (\<lambda>\<tau>. \<theta> (x \<tau>) - \<nu> (x \<tau>)) = (\<lambda>r. \<theta>' (x r) - \<nu>' (x r)) on {0..\<tau>}))"
 shows "(\<lambda>s. \<nu> s < \<theta> s) is_diff_invariant_of f along {0..t}"
 proof(simp add: diff_invariant_def ivp_sols_def, clarsimp)
   fix x \<tau> assume tHyp:"0 \<le> \<tau>" "\<tau> \<le> t"
     and x_ivp:"D x = (\<lambda>\<tau>. f (x \<tau>)) on {0..t}" "\<nu> (x 0) < \<theta> (x 0)"
-  hence primed:"\<forall> r \<in> {0--\<tau>}. ((\<lambda>\<tau>. \<theta> (x \<tau>) - \<nu> (x \<tau>)) has_derivative 
-(\<lambda>\<tau>. \<tau> *\<^sub>R  (\<theta>' (x r) -  \<nu>' (x r)))) (at r within {0--\<tau>}) \<and> \<theta>' (x r) \<ge> \<nu>' (x r)" 
-    using assms by auto
-  hence "\<exists>r\<in>{0--\<tau>}. (\<theta> (x \<tau>) - \<nu> (x \<tau>)) - (\<theta> (x 0) - \<nu> (x 0)) = 
+  hence primed:"\<forall> r \<in> {0..\<tau>}. ((\<lambda>\<tau>. \<theta> (x \<tau>) - \<nu> (x \<tau>)) has_derivative 
+(\<lambda>\<tau>. \<tau> *\<^sub>R  (\<theta>' (x r) -  \<nu>' (x r)))) (at r within {0..\<tau>}) \<and> \<theta>' (x r) \<ge> \<nu>' (x r)" 
+    using assms by (auto simp: has_vderiv_on_def has_vector_derivative_def)
+  hence "\<exists>r\<in>{0..\<tau>}. (\<theta> (x \<tau>) - \<nu> (x \<tau>)) - (\<theta> (x 0) - \<nu> (x 0)) = 
   (\<lambda>\<tau>. \<tau> *\<^sub>R (\<theta>' (x r) -  \<nu>' (x r))) (\<tau> - 0)" 
-    by(rule_tac closed_segment_mvt, auto simp: \<open>0 \<le> \<tau>\<close>)
-  then obtain r where "r \<in> {0--\<tau>}" and 
+    by(rule_tac mvt_very_simple) (auto simp: tHyp)
+  then obtain r where "r \<in> {0..\<tau>}" and 
     "\<theta> (x \<tau>) - \<nu> (x \<tau>) = (\<tau> - 0) *\<^sub>R (\<theta>' (x r) -  \<nu>' (x r)) + (\<theta> (x 0) - \<nu> (x 0))" 
     by force 
   also have "... > 0" 
@@ -409,18 +399,16 @@ proof(simp add: diff_invariant_def ivp_sols_def, clarsimp)
     by simp
 qed
 
-lemma [ode_invariant_rules]:
-fixes \<theta>::"'a::banach \<Rightarrow> real"
-assumes "I1 is_diff_invariant_of f along {0..t}" 
-    and "I2 is_diff_invariant_of f along {0..t}"
-shows "(\<lambda>s. I1 s \<and> I2 s) is_diff_invariant_of f along {0..t}"
+lemma [diff_invariant_rules]:
+assumes "I\<^sub>1 is_diff_invariant_of f along {0..t}" 
+    and "I\<^sub>2 is_diff_invariant_of f along {0..t}"
+shows "(\<lambda>s. I\<^sub>1 s \<and> I\<^sub>2 s) is_diff_invariant_of f along {0..t}"
   using assms unfolding diff_invariant_def by auto
 
-lemma [ode_invariant_rules]:
-fixes \<theta>::"'a::banach \<Rightarrow> real"
-assumes "I1 is_diff_invariant_of f along {0..t}" 
-    and "I2 is_diff_invariant_of f along {0..t}"
-shows "(\<lambda>s. I1 s \<or> I2 s) is_diff_invariant_of f along {0..t}"
+lemma [diff_invariant_rules]:
+assumes "I\<^sub>1 is_diff_invariant_of f along {0..t}" 
+    and "I\<^sub>2 is_diff_invariant_of f along {0..t}"
+shows "(\<lambda>s. I\<^sub>1 s \<or> I\<^sub>2 s) is_diff_invariant_of f along {0..t}"
   using assms unfolding diff_invariant_def by auto
 
 end
