HybridVerifVecs/rels/cat2rel_examples.thy
@@ -6,7 +6,7 @@ begin
 subsection\<open> Examples \<close>
 
 text\<open> The examples in this subsection show different approaches for the verification of hybrid 
-systems. However, the general approach can be outlined as follows: First, we select a finite type to
+systems. however, the general approach can be outlined as follows: First, we select a finite type to
 model program variables @{typ 'n}. We use this to define a vector field @{term f} of type
  @{typ "'a^'n \<Rightarrow> 'a^'n"} to model the dynamics of our system. Then we show a partial correctness 
 specification involving the evolution command @{term "([x\<acute>=f]T & G)"} either by finding a flow for 
@@ -25,9 +25,9 @@ verification easier to parse.
 hybrid program).
 \end{enumerate} \<close>
 
-typedef program_vars ="{''y'',''v''}"
+typedef program_vars ="{''x'',''v''}"
   morphisms to_str to_var
-  apply(rule_tac x="''y''" in exI)
+  apply(rule_tac x="''x''" in exI)
   by simp
 
 notation to_var ("\<restriction>\<^sub>V")
@@ -36,21 +36,21 @@ lemma number_of_program_vars:"CARD(program_vars) = 2"
   using type_definition.card type_definition_program_vars by fastforce
 
 instance program_vars::finite
-  apply(standard, subst bij_betw_finite[of to_str UNIV "{''y'',''v''}"])
+  apply(standard, subst bij_betw_finite[of to_str UNIV "{''x'',''v''}"])
    apply(rule bij_betwI')
      apply (simp add: to_str_inject)
   using to_str apply blast
    apply (metis to_var_inverse UNIV_I)
   by simp
 
-lemma program_vars_univD:"(UNIV::program_vars set) = {\<restriction>\<^sub>V ''y'', \<restriction>\<^sub>V ''v''}"
+lemma program_vars_univD:"(UNIV::program_vars set) = {\<restriction>\<^sub>V ''x'', \<restriction>\<^sub>V ''v''}"
   apply auto by (metis to_str to_str_inverse insertE singletonD) 
 
-lemma program_vars_exhaust:"\<forall>x::program_vars. x = \<restriction>\<^sub>V ''y'' \<or> x = \<restriction>\<^sub>V ''v''"
+lemma program_vars_exhaust:"x = \<restriction>\<^sub>V ''x'' \<or> x = \<restriction>\<^sub>V ''v''"
   using program_vars_univD by auto
 
 abbreviation "constant_acceleration_kinematics g s \<equiv> 
-  (\<chi> i. if i=(\<restriction>\<^sub>V ''y'') then s $ (\<restriction>\<^sub>V ''v'') else g)"
+  (\<chi> i. if i=(\<restriction>\<^sub>V ''x'') then s $ (\<restriction>\<^sub>V ''v'') else g)"
 
 notation constant_acceleration_kinematics ("K")
 
@@ -63,8 +63,8 @@ lemma cnst_acc_continuous:
 
 lemma picard_lindeloef_cnst_acc:
   fixes g::real assumes "0 \<le> t" and "t < 1 "
-  shows "picard_lindeloef (\<lambda>t. K g) {0..t} 1 0"
-  unfolding picard_lindeloef_def apply(simp add: lipschitz_on_def assms, safe)
+  shows "picard_lindeloef_closed_ivl (\<lambda>t. K g) {0..t} 1 0"
+  unfolding picard_lindeloef_closed_ivl_def apply(simp add: lipschitz_on_def assms, safe)
   apply(rule_tac t="UNIV" and f="snd" in continuous_on_compose2)
   apply(simp_all add: cnst_acc_continuous continuous_on_snd)
    apply(simp add: dist_vec_def L2_set_def dist_real_def)
@@ -73,35 +73,31 @@ lemma picard_lindeloef_cnst_acc:
   using assms by linarith
 
 abbreviation "constant_acceleration_kinematics_flow g t s \<equiv> 
-  (\<chi> i. if i=(\<restriction>\<^sub>V ''y'') then g \<cdot> t ^ 2/2 + s $ (\<restriction>\<^sub>V ''v'') \<cdot> t + s $ (\<restriction>\<^sub>V ''y'') 
+  (\<chi> i. if i=(\<restriction>\<^sub>V ''x'') then g \<cdot> t ^ 2/2 + s $ (\<restriction>\<^sub>V ''v'') \<cdot> t + s $ (\<restriction>\<^sub>V ''x'') 
         else g \<cdot> t + s $ (\<restriction>\<^sub>V ''v''))"
 
 notation constant_acceleration_kinematics_flow ("\<phi>\<^sub>K")
+
+term "D (\<lambda>t. \<phi>\<^sub>K g t s) = (\<lambda>t. K g (\<phi>\<^sub>K g t s)) on {0..t}"
 
 lemma local_flow_cnst_acc:
   assumes "0 \<le> t" and "t < 1 "
   shows "local_flow (K g) {0..t} 1 (\<phi>\<^sub>K g)"
   unfolding local_flow_def local_flow_axioms_def apply safe
   using assms picard_lindeloef_cnst_acc apply blast
-   apply(rule has_vderiv_on_vec_lambda)
-  using poly_derivatives(3,4) program_vars_exhaust
-   apply(simp_all add: to_var_inject vec_eq_iff has_vderiv_on_def has_vector_derivative_def)
-  using program_vars_exhaust by blast
-
-lemma wp_cnst_acc:
-  assumes "0 \<le> t" and "t < 1"
-  shows " wp ([x\<acute>=K g]{0..t} & G) \<lceil>Q\<rceil> = 
-    \<lceil>\<lambda> s. \<forall> \<tau> \<in> {0..t}. (G \<rhd> (\<lambda>r. \<phi>\<^sub>K g r s){0--\<tau>}) \<longrightarrow> Q (\<phi>\<^sub>K g \<tau> s)\<rceil>"
-  apply(subst local_flow.wp_g_orbit[of "K g" _ 1 "(\<lambda> t x. \<phi>\<^sub>K g t x)"])
-  using local_flow_cnst_acc and assms by(auto simp: p2r_def)
+   apply(rule has_vderiv_on_vec_lambda, clarify)
+   apply(case_tac "i = \<restriction>\<^sub>V ''x''")
+  using program_vars_exhaust
+  by(auto intro!: poly_derivatives simp: to_var_inject vec_eq_iff)
 
 lemma single_evolution_ball:
-  fixes H::real assumes "0 \<le> t" and "t < 1" and "g < 0"
-  shows "\<lceil>\<lambda>s. 0 \<le> s $ (\<restriction>\<^sub>V ''y'') \<and> s $ (\<restriction>\<^sub>V ''y'') = H \<and> s $ (\<restriction>\<^sub>V ''v'') = 0\<rceil> 
+  fixes h::real assumes "0 \<le> t" and "t < 1" and "g < 0"
+  shows "\<lceil>\<lambda>s. 0 \<le> s $ (\<restriction>\<^sub>V ''y'') \<and> s $ (\<restriction>\<^sub>V ''y'') = h \<and> s $ (\<restriction>\<^sub>V ''v'') = 0\<rceil> 
   \<le> wp ([x\<acute>=K g]{0..t} & (\<lambda> s. s $ (\<restriction>\<^sub>V ''y'') \<ge> 0))
-  \<lceil>\<lambda>s. 0 \<le> s $ (\<restriction>\<^sub>V ''y'') \<and> s $ (\<restriction>\<^sub>V ''y'') \<le> H\<rceil>"
-  apply(subst wp_cnst_acc)
-  using assms by(auto simp: mult_nonpos_nonneg)
+  \<lceil>\<lambda>s. 0 \<le> s $ (\<restriction>\<^sub>V ''y'') \<and> s $ (\<restriction>\<^sub>V ''y'') \<le> h\<rceil>"
+  apply(subst local_flow.wp_g_orbit[OF local_flow_cnst_acc])
+  using assms by (auto simp: mult_nonneg_nonpos2) 
+    (metis (full_types) less_eq_real_def program_vars_exhaust split_mult_neg_le)
 
 no_notation to_var ("\<restriction>\<^sub>V")
 
@@ -127,7 +123,7 @@ lemma "CARD(program_vars) = CARD(2)"
   unfolding number_of_program_vars by simp
 
 text \<open>In fact, for each natural number $n$ there is already a corresponding $n$-element type in 
-Isabelle. However, there are still lemmas to prove about them in order to do verification of hybrid
+Isabelle. however, there are still lemmas to prove about them in order to do verification of hybrid
 systems in $n$-dimensional Euclidean spaces.\<close>
 
 lemma exhaust_5: \<comment> \<open>The analogs for $1,2$ and $3$ have already been proven in Analysis.\<close>
@@ -154,52 +150,42 @@ lemma "\<e> 1 = (\<chi> j::3. if j= 0 then 0 else if j = 1 then 1 else 0)"
   unfolding axis_def by(rule Cart_lambda_cong, simp)
 
 abbreviation "constant_acceleration_kinematics_matrix \<equiv> 
-  (\<chi> i. if i= (0::3) then axis (1::3) (1::real) else if i= 1 then axis 2 1 else 0)"
+  (\<chi> i::3. if i=0 then \<e> 1 else if i=1 then \<e> 2 else (0::real^3))"
 
 abbreviation "constant_acceleration_kinematics_matrix_flow t s \<equiv> 
-  (\<chi> i. if i= (0::3) then s $ 2 \<cdot> t ^ 2/2 + s $ 1 \<cdot> t + s $ 0
+  (\<chi> i::3. if i=0 then s $ 2 \<cdot> t ^ 2/2 + s $ 1 \<cdot> t + s $ 0
    else if i=1 then s $ 2 \<cdot> t + s $ 1 else s $ 2)"
 
-notation constant_acceleration_kinematics_matrix ("K")
+notation constant_acceleration_kinematics_matrix ("A")
 
-notation constant_acceleration_kinematics_matrix_flow ("\<phi>\<^sub>K")
+notation constant_acceleration_kinematics_matrix_flow ("\<phi>\<^sub>A")
 
 text\<open> With these 2 definitions and the proof that linear systems of ODEs are Picard-Lindeloef, we 
 can show that they form a pair of vector-field and its flow. \<close>
 
-lemma entries_cnst_acc_matrix: "entries K = {0, 1}"
+lemma entries_cnst_acc_matrix: "entries A = {0, 1}"
   apply (simp_all add: axis_def, safe)
   by(rule_tac x="1" in exI, simp)+
 
-lemma picard_lindeloef_cnst_acc_matrix:
-  assumes "0 \<le> t" and "t < 1/9"
-  shows "picard_lindeloef (\<lambda> t s. K *v s) {0..t} ((real CARD(3))\<^sup>2 \<cdot> (\<parallel>K\<parallel>\<^sub>m\<^sub>a\<^sub>x)) 0"
-  apply(rule picard_lindeloef_linear_system)
-  unfolding entries_cnst_acc_matrix using assms by auto
-
 lemma local_flow_cnst_acc_matrix:
   assumes "0 \<le> t" and "t < 1/9"
-  shows "local_flow ((*v) K) {0..t} ((real CARD(3))\<^sup>2 \<cdot> (\<parallel>K\<parallel>\<^sub>m\<^sub>a\<^sub>x)) \<phi>\<^sub>K"
+  shows "local_flow ((*v) A) {0..t} ((real CARD(3))\<^sup>2 \<cdot> (\<parallel>A\<parallel>\<^sub>m\<^sub>a\<^sub>x)) \<phi>\<^sub>A"
   unfolding local_flow_def local_flow_axioms_def apply safe
-  using picard_lindeloef_cnst_acc_matrix[OF assms] apply blast
+    apply(rule picard_lindeloef_linear_system[where A=A and t=t])
+  using entries_cnst_acc_matrix assms apply(force, simp, force)
    apply(rule has_vderiv_on_vec_lambda)
-  using poly_derivatives(1,3, 4) 
-   apply(force simp: matrix_vector_mult_def)
-  using exhaust_3 by(force simp: matrix_vector_mult_def vec_eq_iff)
+   apply(auto intro!: poly_derivatives simp: matrix_vector_mult_def vec_eq_iff)
+  using exhaust_3 by force
 
 text\<open> Finally, we compute the wlp of this example and use it to verify the single-evolution ball again.\<close>
 
-lemma wp_cnst_acc_matrix:
-  assumes "0 \<le> t" and "t < 1/9"
-  shows "wp ([x\<acute>=(*v) K]{0..t} & G) \<lceil>Q\<rceil> = \<lceil>\<lambda> s. \<forall>\<tau>\<in>{0..t}. (G \<rhd> (\<lambda>r. \<phi>\<^sub>K r s){0--\<tau>}) \<longrightarrow> Q (\<phi>\<^sub>K \<tau> s)\<rceil>"
-  apply(subst local_flow.wp_g_orbit[of "(*v) K" _ "((real CARD(3))\<^sup>2 \<cdot> (\<parallel>K\<parallel>\<^sub>m\<^sub>a\<^sub>x))" "\<phi>\<^sub>K"])
-  using local_flow_cnst_acc_matrix and assms by auto
-
 lemma single_evolution_ball_K:
   assumes "0 \<le> t" and "t < 1/9" 
-  shows "\<lceil>\<lambda>s. 0 \<le> s $ 0 \<and> s $ 0 = H \<and> s $ 1 = 0 \<and> 0 > s $ 2\<rceil> 
-  \<le> wp ([x\<acute>=(*v) K]{0..t} & (\<lambda>s. s $ 0 \<ge> 0)) \<lceil>\<lambda>s. 0 \<le> s $ 0 \<and> s $ 0 \<le> H\<rceil>"
-  apply(subst wp_cnst_acc_matrix)
+  shows "\<lceil>\<lambda>s. 0 \<le> s $ 0 \<and> s $ 0 = h \<and> s $ 1 = 0 \<and> 0 > s $ 2\<rceil> 
+  \<le> wp ([x\<acute>=(*v) A]{0..t} & (\<lambda>s. s $ 0 \<ge> 0)) 
+  \<lceil>\<lambda>s. 0 \<le> s $ 0 \<and> s $ 0 \<le> h\<rceil>"
+  apply(subst local_flow.wp_g_orbit[of _ _ "9 \<cdot> (\<parallel>A\<parallel>\<^sub>m\<^sub>a\<^sub>x)" \<phi>\<^sub>A])
+  using local_flow_cnst_acc_matrix and assms apply force
   using assms by(auto simp: mult_nonneg_nonpos2)
 
 
@@ -219,42 +205,31 @@ linear operator and the specification is proven again with this flow.
 lemma two_eq_zero: "(2::2) = 0" 
   by simp
 
-lemma [simp]:"i \<noteq> (0::2) \<longrightarrow> i = 1" 
+lemma [simp]: "i \<noteq> (0::2) \<longrightarrow> i = 1" 
   using exhaust_2 by fastforce
 
-lemma UNIV_2:"(UNIV::2 set) = {0, 1}"
+lemma UNIV_2: "(UNIV::2 set) = {0, 1}"
   apply safe using exhaust_2 two_eq_zero by auto
 
-abbreviation "circular_motion_matrix \<equiv> 
-  (\<chi> i. if i= (0::2) then axis (1::2) (- 1::real) else axis 0 1)"
+abbreviation circular_motion_matrix :: "real^2^2" 
+  where "circular_motion_matrix \<equiv> (\<chi> i. if i=0 then - \<e> 1 else \<e> 0)"
 
 notation circular_motion_matrix ("C")
 
 lemma circle_invariant:
-  assumes "0 < R"
-  shows "(\<lambda>s. R\<^sup>2 = (s $ 0)\<^sup>2 + (s $ 1)\<^sup>2) is_diff_invariant_of (*v) C along {0..t}"
-  apply(rule_tac ode_invariant_rules, clarsimp)
+  shows "(\<lambda>s. r\<^sup>2 = (s $ 0)\<^sup>2 + (s $ 1)\<^sup>2) is_diff_invariant_of (*v) C along {0..t}"
+  apply(rule_tac diff_invariant_rules, clarsimp)
   apply(frule_tac i="0" in has_vderiv_on_vec_nth, drule_tac i="1" in has_vderiv_on_vec_nth)
-  apply(unfold has_vderiv_on_def has_vector_derivative_def, clarsimp)
-  apply(erule_tac x="r" in ballE)+
-    apply(simp add: matrix_vector_mult_def has_vderiv_on_vec_lambda)
-  subgoal for x \<tau> r apply(rule_tac f'1="\<lambda>t. 0" and g'1="\<lambda>t. 0" in derivative_eq_intros(11), simp_all)
-     apply(rule_tac f'1="\<lambda>t. - 2 \<cdot> (x r $ 0) \<cdot> (t \<cdot> x r $ 1)" 
-        and g'1="\<lambda>t. 2 \<cdot> (x r $ 1) \<cdot> t \<cdot> x r $ 0" in derivative_eq_intros(8), simp_all)
-       apply(rule_tac f'1="\<lambda>t. - (t \<cdot> x r $ 1)" in derivative_eq_intros(15))
-        apply(rule_tac t="{0--\<tau>}" and s="{0..t}" in has_derivative_within_subset)
-         apply(simp, simp add: closed_segment_eq_real_ivl, force)
-       apply(rule_tac f'1="\<lambda>t. (t \<cdot> x r $ 0)" in derivative_eq_intros(15))
-        apply(rule_tac t="{0--\<tau>}" and s="{0..t}" in has_derivative_within_subset)
-    by(simp, simp add: closed_segment_eq_real_ivl, force)
-  by(auto simp: closed_segment_eq_real_ivl)
+  apply(rule_tac S="{0..t}" in has_vderiv_on_subset)
+  by(auto intro!: poly_derivatives simp: matrix_vector_mult_def)
 
 lemma circular_motion_invariants:
-  assumes "(R::real) > 0"
-  shows "\<lceil>\<lambda>s. R\<^sup>2 = (s $ 0)\<^sup>2 + (s $ 1)\<^sup>2\<rceil> \<le> wp ([x\<acute>=(*v) C]{0..t} & G) \<lceil>\<lambda>s. R\<^sup>2 = (s $ 0)\<^sup>2 + (s $ 1)\<^sup>2\<rceil>"
-  using assms(1) apply(rule_tac C="\<lambda>s. R\<^sup>2 = (s $ 0)\<^sup>2 + (s $ 1)\<^sup>2" in dCut)
-   apply(rule_tac I="\<lambda>s. R\<^sup>2 = (s $ 0)\<^sup>2 + (s $ 1)\<^sup>2" in dI)
-  using circle_invariant \<open>R > 0\<close> apply(blast, force, force)
+  shows "\<lceil>\<lambda>s. r\<^sup>2 = (s $ 0)\<^sup>2 + (s $ 1)\<^sup>2\<rceil> \<le> 
+  wp ([x\<acute>=(*v) C]{0..t} & G) 
+  \<lceil>\<lambda>s. r\<^sup>2 = (s $ 0)\<^sup>2 + (s $ 1)\<^sup>2\<rceil>"
+  apply(rule_tac C="\<lambda>s. r\<^sup>2 = (s $ 0)\<^sup>2 + (s $ 1)\<^sup>2" in dCut)
+   apply(rule_tac I="\<lambda>s. r\<^sup>2 = (s $ 0)\<^sup>2 + (s $ 1)\<^sup>2" in dI)
+  using circle_invariant apply(blast, force, force)
   by(rule dWeakening, auto)
 
 \<comment> \<open>Proof of the same specification by providing solutions:\<close>
@@ -265,14 +240,8 @@ lemma entries_circ_matrix:"entries C = {0, - 1, 1}"
   subgoal by(rule_tac x="0" in exI, simp)+
   by(rule_tac x="1" in exI, simp)+
 
-lemma picard_lindeloef_circ_matrix:
-  assumes "0 \<le> t" and "t < 1/4" 
-  shows "picard_lindeloef (\<lambda>t. (*v) C) {0..t} ((real CARD(2))\<^sup>2 \<cdot> (\<parallel>C\<parallel>\<^sub>m\<^sub>a\<^sub>x)) 0"
-  apply(rule picard_lindeloef_linear_system)
-  unfolding entries_circ_matrix using assms by auto
-
-abbreviation "circular_motion_matrix_flow t s \<equiv> (\<chi> i. if i= (0::2) then 
-s$0 \<cdot> cos t - s$1 \<cdot> sin t else s$0 \<cdot> sin t + s$1 \<cdot> cos t)"
+abbreviation "circular_motion_matrix_flow t s \<equiv> 
+  (\<chi> i::2. if i=0 then s$0 \<cdot> cos t - s$1 \<cdot> sin t else s$0 \<cdot> sin t + s$1 \<cdot> cos t)"
 
 notation circular_motion_matrix_flow ("\<phi>\<^sub>C")
 
@@ -280,40 +249,18 @@ lemma local_flow_circ_mtx:
   assumes "0 \<le> t" and "t < 1/4" 
   shows "local_flow ((*v) C) {0..t} ((real CARD(2))\<^sup>2 \<cdot> (\<parallel>C\<parallel>\<^sub>m\<^sub>a\<^sub>x)) \<phi>\<^sub>C"
   unfolding local_flow_def local_flow_axioms_def apply safe
-  using picard_lindeloef_circ_matrix assms apply blast
+    apply(rule picard_lindeloef_linear_system)
+  unfolding entries_circ_matrix using assms apply(simp_all)
    apply(rule has_vderiv_on_vec_lambda)
-   apply(simp add: matrix_vector_mult_def has_vderiv_on_def has_vector_derivative_def, safe)
-  subgoal for s i x
-    apply(rule_tac f'1="\<lambda>t. - s$0 \<cdot> (t \<cdot> sin x)" and g'1="\<lambda>t. s$1 \<cdot> (t \<cdot> cos x)"in derivative_eq_intros(11))
-      apply(rule derivative_eq_intros(6)[of cos "(\<lambda>xa. - (xa \<cdot> sin x))"])
-       apply(rule_tac Db1="1" in derivative_eq_intros(58))
-        apply(rule ssubst[of "(\<cdot>) 1" id], force, simp, force, force)
-     apply(rule derivative_eq_intros(6)[of sin "(\<lambda>xa. (xa \<cdot> cos x))"])
-      apply(rule_tac Db1="1" in derivative_eq_intros(55))
-       apply(rule ssubst[of "(\<cdot>) 1" id], force, simp, force, force)
-    by (simp add: Groups.mult_ac(3) Rings.ring_distribs(4))
-  subgoal for s i x
-    apply(rule_tac f'1="\<lambda>t. s$0 \<cdot> (t \<cdot> cos x)" and g'1="\<lambda>t. - s$1 \<cdot> (t \<cdot> sin x)"in derivative_eq_intros(8))
-      apply(rule derivative_eq_intros(6)[of sin "(\<lambda>xa. xa \<cdot> cos x)"])
-       apply(rule_tac Db1="1" in derivative_eq_intros(55))
-        apply(rule ssubst[of "(\<cdot>) 1" id], force, simp, force, force)
-     apply(rule derivative_eq_intros(6)[of cos "(\<lambda>xa. - (xa \<cdot> sin x))"])
-      apply(rule_tac Db1="1" in derivative_eq_intros(58))
-       apply(rule ssubst[of "(\<cdot>) 1" id], force, simp, force, force)
-    by (simp add: Groups.mult_ac(3) Rings.ring_distribs(4))
+  apply(force intro!: poly_derivatives simp: matrix_vector_mult_def)
   using exhaust_2 two_eq_zero by(force simp: vec_eq_iff)
 
-lemma flow_for_Circ_DS:
-  assumes "0 \<le> t" and "t < 1/4"
-  shows " wp ([x\<acute>=(*v) C]{0..t} & G) \<lceil>Q\<rceil> = 
-    \<lceil>\<lambda> x. \<forall> \<tau> \<in> {0..t}. (\<forall>r\<in>{0--\<tau>}. G (\<phi>\<^sub>C r x)) \<longrightarrow> Q (\<phi>\<^sub>C \<tau> x)\<rceil>"
-  apply(subst local_flow.wp_g_orbit[of "(*v) C" _ "((real CARD(2))\<^sup>2 \<cdot> (\<parallel>C\<parallel>\<^sub>m\<^sub>a\<^sub>x))" \<phi>\<^sub>C])
-  using local_flow_circ_mtx and assms by auto
-
 lemma circular_motion:
-  assumes "0 \<le> t" and "t < 1/4" and "R > 0"
-  shows "\<lceil>\<lambda>s. R\<^sup>2 = (s $ 0)\<^sup>2 + (s $ 1)\<^sup>2\<rceil> \<le> wp ([x\<acute>=(*v) C]{0..t} & G) \<lceil>\<lambda>s. R\<^sup>2 = (s $ 0)\<^sup>2 + (s $ 1)\<^sup>2\<rceil>"
-  apply(subst flow_for_Circ_DS)
+  assumes "0 \<le> t" and "t < 1/4"
+  shows "\<lceil>\<lambda>s. r\<^sup>2 = (s $ 0)\<^sup>2 + (s $ 1)\<^sup>2\<rceil> \<le>
+   wp ([x\<acute>=(*v) C]{0..t} & G) 
+  \<lceil>\<lambda>s. r\<^sup>2 = (s $ 0)\<^sup>2 + (s $ 1)\<^sup>2\<rceil>"
+  apply(subst local_flow.wp_g_orbit[OF local_flow_circ_mtx])
   using assms by simp_all
 
 no_notation circular_motion_matrix ("C")
@@ -331,55 +278,55 @@ arithmetic. \<close>
 
 named_theorems bb_real_arith "real arithmetic properties for the bouncing ball."
 
-lemma [bb_real_arith]:"0 \<le> x \<Longrightarrow> 0 > g \<Longrightarrow> 2 \<cdot> g \<cdot> x = 2 \<cdot> g \<cdot> H + v \<cdot> v \<Longrightarrow> (x::real) \<le> H"
+lemma [bb_real_arith]: "0 \<le> x \<Longrightarrow> 0 > g \<Longrightarrow> 2 \<cdot> g \<cdot> x = 2 \<cdot> g \<cdot> h + v \<cdot> v \<Longrightarrow> (x::real) \<le> h"
 proof-
-  assume "0 \<le> x" and "0 > g" and "2 \<cdot> g \<cdot> x = 2 \<cdot> g \<cdot> H + v \<cdot> v"
-  then have "v \<cdot> v = 2 \<cdot> g \<cdot> x - 2 \<cdot> g \<cdot> H \<and> 0 > g" by auto
-  hence *:"v \<cdot> v = 2 \<cdot> g \<cdot> (x - H) \<and> 0 > g \<and> v \<cdot> v \<ge> 0" 
+  assume "0 \<le> x" and "0 > g" and "2 \<cdot> g \<cdot> x = 2 \<cdot> g \<cdot> h + v \<cdot> v"
+  then have "v \<cdot> v = 2 \<cdot> g \<cdot> x - 2 \<cdot> g \<cdot> h \<and> 0 > g" by auto
+  hence *:"v \<cdot> v = 2 \<cdot> g \<cdot> (x - h) \<and> 0 > g \<and> v \<cdot> v \<ge> 0" 
     using left_diff_distrib mult.commute by (metis zero_le_square) 
-  from this have "(v \<cdot> v)/(2 \<cdot> g) = (x - H)" by auto 
+  from this have "(v \<cdot> v)/(2 \<cdot> g) = (x - h)" by auto 
   also from * have "(v \<cdot> v)/(2 \<cdot> g) \<le> 0"
     using divide_nonneg_neg by fastforce 
-  ultimately have "H - x \<ge> 0" by linarith
+  ultimately have "h - x \<ge> 0" by linarith
   thus ?thesis by auto
 qed
 
 lemma [bb_real_arith]:
-  assumes invar:"2 \<cdot> g \<cdot> x = 2 \<cdot> g \<cdot> H + v \<cdot> v"
-    and pos:"g \<cdot> \<tau>\<^sup>2 / 2 + v \<cdot> \<tau> + (x::real) = 0"
-  shows "2 \<cdot> g \<cdot> H + (- (g \<cdot> \<tau>) - v) \<cdot> (- (g \<cdot> \<tau>) - v) = 0"
-and "2 \<cdot> g \<cdot> H + (g \<cdot> \<tau> \<cdot> (g \<cdot> \<tau> + v) + v \<cdot> (g \<cdot> \<tau> + v)) = 0"
+  assumes invar: "2 \<cdot> g \<cdot> x = 2 \<cdot> g \<cdot> h + v \<cdot> v"
+    and pos: "g \<cdot> \<tau>\<^sup>2 / 2 + v \<cdot> \<tau> + (x::real) = 0"
+  shows "2 \<cdot> g \<cdot> h + (- (g \<cdot> \<tau>) - v) \<cdot> (- (g \<cdot> \<tau>) - v) = 0"
+and "2 \<cdot> g \<cdot> h + (g \<cdot> \<tau> \<cdot> (g \<cdot> \<tau> + v) + v \<cdot> (g \<cdot> \<tau> + v)) = 0"
 proof-
   from pos have "g \<cdot> \<tau>\<^sup>2  + 2 \<cdot> v \<cdot> \<tau> + 2 \<cdot> x = 0" by auto
   then have "g\<^sup>2  \<cdot> \<tau>\<^sup>2  + 2 \<cdot> g \<cdot> v \<cdot> \<tau> + 2 \<cdot> g \<cdot> x = 0"
     by (metis (mono_tags, hide_lams) Groups.mult_ac(1,3) mult_zero_right
         monoid_mult_class.power2_eq_square semiring_class.distrib_left)
-  hence "g\<^sup>2 \<cdot> \<tau>\<^sup>2 + 2 \<cdot> g \<cdot> v \<cdot> \<tau> + v\<^sup>2 + 2 \<cdot> g \<cdot> H = 0"
+  hence "g\<^sup>2 \<cdot> \<tau>\<^sup>2 + 2 \<cdot> g \<cdot> v \<cdot> \<tau> + v\<^sup>2 + 2 \<cdot> g \<cdot> h = 0"
     using invar by (simp add: monoid_mult_class.power2_eq_square) 
-  from this have *:"(g \<cdot> \<tau> + v)\<^sup>2 + 2 \<cdot> g \<cdot> H = 0"
+  from this have *:"(g \<cdot> \<tau> + v)\<^sup>2 + 2 \<cdot> g \<cdot> h = 0"
     apply(subst power2_sum) by (metis (no_types, hide_lams) Groups.add_ac(2, 3) 
         Groups.mult_ac(2, 3) monoid_mult_class.power2_eq_square nat_distrib(2))
-  hence "2 \<cdot> g \<cdot> H + (- ((g \<cdot> \<tau>) + v))\<^sup>2 = 0"
+  hence "2 \<cdot> g \<cdot> h + (- ((g \<cdot> \<tau>) + v))\<^sup>2 = 0"
     by (metis Groups.add_ac(2) power2_minus)
-  thus "2 \<cdot> g \<cdot> H + (- (g \<cdot> \<tau>) - v) \<cdot> (- (g \<cdot> \<tau>) - v) = 0"
+  thus "2 \<cdot> g \<cdot> h + (- (g \<cdot> \<tau>) - v) \<cdot> (- (g \<cdot> \<tau>) - v) = 0"
     by (simp add: monoid_mult_class.power2_eq_square)
-  from * show "2 \<cdot> g \<cdot> H + (g \<cdot> \<tau> \<cdot> (g \<cdot> \<tau> + v) + v \<cdot> (g \<cdot> \<tau> + v)) = 0"
+  from * show "2 \<cdot> g \<cdot> h + (g \<cdot> \<tau> \<cdot> (g \<cdot> \<tau> + v) + v \<cdot> (g \<cdot> \<tau> + v)) = 0"
     by (simp add: monoid_mult_class.power2_eq_square)
 qed
     
 lemma [bb_real_arith]:
-  assumes invar:"2 \<cdot> g \<cdot> x = 2 \<cdot> g \<cdot> H + v \<cdot> v"
+  assumes invar: "2 \<cdot> g \<cdot> x = 2 \<cdot> g \<cdot> h + v \<cdot> v"
   shows "2 \<cdot> g \<cdot> (g \<cdot> \<tau>\<^sup>2 / 2 + v \<cdot> \<tau> + (x::real)) = 
-  2 \<cdot> g \<cdot> H + (g \<cdot> \<tau> \<cdot> (g \<cdot> \<tau> + v) + v \<cdot> (g \<cdot> \<tau> + v))" (is "?lhs = ?rhs")
+  2 \<cdot> g \<cdot> h + (g \<cdot> \<tau> \<cdot> (g \<cdot> \<tau> + v) + v \<cdot> (g \<cdot> \<tau> + v))" (is "?lhs = ?rhs")
 proof-
   have "?lhs = g\<^sup>2 \<cdot> \<tau>\<^sup>2 + 2 \<cdot> g \<cdot> v \<cdot> \<tau> + 2 \<cdot> g \<cdot> x"
     apply(subst Rat.sign_simps(18))+
     by(auto simp: semiring_normalization_rules(29))
-  also have "... = g\<^sup>2 \<cdot> \<tau>\<^sup>2 + 2 \<cdot> g \<cdot> v \<cdot> \<tau> + 2 \<cdot> g \<cdot> H + v \<cdot> v" (is "... = ?middle")
+  also have "... = g\<^sup>2 \<cdot> \<tau>\<^sup>2 + 2 \<cdot> g \<cdot> v \<cdot> \<tau> + 2 \<cdot> g \<cdot> h + v \<cdot> v" (is "... = ?middle")
     by(subst invar, simp)
   finally have "?lhs = ?middle".
   moreover 
-  {have "?rhs = g \<cdot> g \<cdot> (\<tau> \<cdot> \<tau>) + 2 \<cdot> g \<cdot> v \<cdot> \<tau> + 2 \<cdot> g \<cdot> H + v \<cdot> v"
+  {have "?rhs = g \<cdot> g \<cdot> (\<tau> \<cdot> \<tau>) + 2 \<cdot> g \<cdot> v \<cdot> \<tau> + 2 \<cdot> g \<cdot> h + v \<cdot> v"
       by (simp add: Groups.mult_ac(2,3) semiring_class.distrib_left)
     also have "... = ?middle"
       by (simp add: semiring_normalization_rules(29))
@@ -389,15 +336,17 @@ qed
 
 lemma bouncing_ball:
   assumes "0 \<le> t" and "t < 1/9" 
-  shows "\<lceil>\<lambda>s. (0::real) \<le> s $ (0::3) \<and> s $ 0 = H \<and> s $ 1 = 0 \<and> 0 > s $ 2\<rceil> \<subseteq> wp 
-  ((([x\<acute>=\<lambda>s. K *v s]{0..t} & (\<lambda> s. s $ 0 \<ge> 0));
-  (IF (\<lambda> s. s $ 0 = 0) THEN ([1 ::== (\<lambda>s. - s $ 1)]) ELSE Id FI))\<^sup>*)
-  \<lceil>\<lambda>s. 0 \<le> s $ 0 \<and> s $ 0 \<le> H\<rceil>"
+  shows "\<lceil>\<lambda>s. 0 \<le> s $ 0 \<and> s $ 0 = h \<and> s $ 1 = 0 \<and> 0 > s $ 2\<rceil> \<subseteq> wp 
+  ((([x\<acute>=\<lambda>s. A *v s]{0..t} & (\<lambda> s. s $ 0 \<ge> 0));
+  (IF (\<lambda> s. s $ 0 = 0) THEN (1 ::= (\<lambda>s. - s $ 1)) ELSE Id FI))\<^sup>*)
+  \<lceil>\<lambda>s. 0 \<le> s $ 0 \<and> s $ 0 \<le> h\<rceil>"
   apply(rule rel_ad_mka_starI [of _ "\<lceil>\<lambda>s. 0 \<le> s $ (0::3) \<and> 0 > s $ 2 \<and> 
-  2 \<cdot> s $ 2 \<cdot> s $ 0 = 2 \<cdot> s $ 2 \<cdot> H + (s $ 1 \<cdot> s $ 1)\<rceil>"])
+  2 \<cdot> s $ 2 \<cdot> s $ 0 = 2 \<cdot> s $ 2 \<cdot> h + (s $ 1 \<cdot> s $ 1)\<rceil>"])
     apply(simp, simp only: rel_antidomain_kleene_algebra.fbox_seq)
-   apply(subst p2r_r2p_wp_sym[of "(IF (\<lambda>s. s $ 0 = 0) THEN ([1 ::== (\<lambda>s. - s $ 1)]) ELSE Id FI)"])
-   apply(subst wp_cnst_acc_matrix) using assms apply(simp, simp) apply(subst wp_trafo) 
+   apply(subst p2r_r2p_wp[symmetric, of "(IF (\<lambda>s. s $ 0 = 0) THEN (1 ::= (\<lambda>s. - s $ 1)) ELSE Id FI)"])
+   apply(subst local_flow.wp_g_orbit[of _ _ "9 \<cdot> (\<parallel>A\<parallel>\<^sub>m\<^sub>a\<^sub>x)" \<phi>\<^sub>A])
+  using local_flow_cnst_acc_matrix[OF assms] apply force
+  apply(subst wp_trafo)
   unfolding rel_antidomain_kleene_algebra.cond_def rel_antidomain_kleene_algebra.ads_d_def 
   by(auto simp: p2r_def rel_ad_def bb_real_arith)
 
@@ -405,51 +354,44 @@ subsubsection\<open> Bouncing Ball with invariants \<close>
 
 text\<open> We prove again the bouncing ball but this time with differential invariants. \<close>
 
-lemma gravity_invariant: "(\<lambda>s. s $ 2 < 0) is_diff_invariant_of (*v) K along {0..t}"
-  apply(rule_tac \<theta>'="\<lambda>s. 0" and \<nu>'="\<lambda>s. 0" in ode_invariant_rules(3), clarsimp)
+lemma gravity_invariant: "(\<lambda>s. s $ 2 < 0) is_diff_invariant_of (*v) A along {0..t}"
+  apply(rule_tac \<theta>'="\<lambda>s. 0" and \<nu>'="\<lambda>s. 0" in diff_invariant_rules(3), clarsimp)
   apply(drule_tac i="2" in has_vderiv_on_vec_nth)
-  apply(unfold has_vderiv_on_def has_vector_derivative_def)
-  apply(erule_tac x="r" in ballE, simp add: matrix_vector_mult_def)
-   apply(rule_tac f'1="\<lambda>s. 0" in derivative_eq_intros(10))
-  by(auto simp: closed_segment_eq_real_ivl has_derivative_within_subset)
+  apply(rule_tac S="{0..t}" in has_vderiv_on_subset)
+  by(auto intro!: poly_derivatives simp: vec_eq_iff matrix_vector_mult_def)
 
 lemma energy_conservation_invariant: 
-"(\<lambda>s. 2 \<cdot> s $ 2 \<cdot> s $ 0 - 2 \<cdot> s $ 2 \<cdot> H - s $ 1 \<cdot> s $ 1 = 0) is_diff_invariant_of (*v) K along {0..t}"
-  apply(rule ode_invariant_rules, clarify)
+  "(\<lambda>s. 2 \<cdot> s$2 \<cdot> s$0 - 2 \<cdot> s$2 \<cdot> h - s$1 \<cdot> s $ 1 = 0) is_diff_invariant_of (*v) A along {0..t}"
+  apply(rule diff_invariant_rules, clarify)
   apply(frule_tac i="2" in has_vderiv_on_vec_nth)
   apply(frule_tac i="1" in has_vderiv_on_vec_nth)
   apply(drule_tac i="0" in has_vderiv_on_vec_nth)
-  apply(unfold has_vderiv_on_def has_vector_derivative_def)
-  apply(erule_tac x="r" in ballE, simp_all add: matrix_vector_mult_def)+
-     apply(rule_tac f'1="\<lambda>t. 2 \<cdot> x r $ 2 \<cdot> (t \<cdot> x r $ 1)" 
-      and g'1="\<lambda>t. 2 \<cdot> (t \<cdot> (x r $ 1 \<cdot> x r $ 2))" in derivative_eq_intros(11))
-     apply(rule_tac f'1="\<lambda>t. 2 \<cdot> x r $ 2 \<cdot> (t \<cdot> x r $ 1)" and g'1="\<lambda>t. 0" in derivative_eq_intros(11))
-     apply(rule_tac f'1="\<lambda>t. 0" and g'1="(\<lambda>xa. xa \<cdot> x r $ 1)" in derivative_eq_intros(12))
-     apply(rule_tac g'1="\<lambda>t. 0" in derivative_eq_intros(6))
-     apply(simp_all add: has_derivative_within_subset closed_segment_eq_real_ivl)
-     apply(rule_tac g'1="\<lambda>t. 0" in derivative_eq_intros(7))
-    apply(rule_tac g'1="\<lambda>t. 0" in derivative_eq_intros(6))
-     apply(simp_all add: has_derivative_within_subset)
-  apply(rule_tac f'1="(\<lambda>xa. xa \<cdot> x r $ 2)" and g'1="(\<lambda>xa. xa \<cdot> x r $ 2)" in derivative_eq_intros(12))
-  by(simp_all add: has_derivative_within_subset)
+  apply(rule_tac S="{0..t}" in has_vderiv_on_subset)
+  by(auto intro!: poly_derivatives simp: vec_eq_iff matrix_vector_mult_def)
 
 lemma bouncing_ball_invariants: 
-  "\<lceil>\<lambda>s. (0::real) \<le> s $ (0::3) \<and> s $ 0 = H \<and> s $ 1 = 0 \<and> 0 > s $ 2\<rceil> \<subseteq> wp 
-  ((([x\<acute>=\<lambda>s. K *v s]{0..t} & (\<lambda> s. s $ 0 \<ge> 0));
-  (IF (\<lambda> s. s $ 0 = 0) THEN ([1 ::== (\<lambda>s. - s $ 1)]) ELSE Id FI))\<^sup>*)
-  \<lceil>\<lambda>s. 0 \<le> s $ 0 \<and> s $ 0 \<le> H\<rceil>"
-  apply(rule_tac I="\<lceil>\<lambda>s. 0 \<le> s$0 \<and> 0 > s$2 \<and> 2 \<cdot> s$2 \<cdot> s$0 = 2 \<cdot> s$2 \<cdot> H + (s$1 \<cdot> s$1)\<rceil>" in rel_ad_mka_starI)
+  "\<lceil>\<lambda>s. 0 \<le> s $ 0 \<and> s $ 0 = h \<and> s $ 1 = 0 \<and> 0 > s $ 2\<rceil> \<subseteq> wp 
+  ((([x\<acute>=\<lambda>s. A *v s]{0..t} & (\<lambda> s. s $ 0 \<ge> 0));
+  (IF (\<lambda> s. s $ 0 = 0) THEN (1 ::= (\<lambda>s. - s $ 1)) ELSE Id FI))\<^sup>*)
+  \<lceil>\<lambda>s. 0 \<le> s $ 0 \<and> s $ 0 \<le> h\<rceil>"
+  apply(rule_tac I="\<lceil>\<lambda>s. 0 \<le> s$0 \<and> 0 > s$2 \<and> 2 \<cdot> s$2 \<cdot> s$0 = 2 \<cdot> s$2 \<cdot> h + (s$1 \<cdot> s$1)\<rceil>" in rel_ad_mka_starI)
     apply(simp, simp only: rel_antidomain_kleene_algebra.fbox_seq)
-   apply(subst p2r_r2p_wp_sym[of "(IF (\<lambda>s. s $ 0 = 0) THEN ([1 ::== (\<lambda>s. - s $ 1)]) ELSE Id FI)"])
+   apply(subst p2r_r2p_wp[symmetric, of "(IF (\<lambda>s. s $ 0 = 0) THEN (1 ::= (\<lambda>s. - s $ 1)) ELSE Id FI)"])
    apply(rule dCut[where C="\<lambda> s. s $ 2 < 0"])
     apply(rule_tac I="\<lambda> s. s $ 2 < 0" in dI)
-  using gravity_invariant apply(blast, force simp: p2r_def, force simp: p2r_def)
-   apply(rule_tac C="\<lambda> s. 2 \<cdot> s$2 \<cdot> s$0 - 2 \<cdot> s$2 \<cdot> H - s$1 \<cdot> s$1 = 0" in dCut)
-    apply(rule_tac I="\<lambda> s. 2 \<cdot> s$2 \<cdot> s$0 - 2 \<cdot> s$2 \<cdot> H - s$1 \<cdot> s$1 = 0" in dI)
-  using energy_conservation_invariant apply(blast, force simp: p2r_def, force simp: p2r_def)
+  using gravity_invariant apply blast
+     apply(force simp: p2r_def, force simp: p2r_def)
+   apply(rule_tac C="\<lambda> s. 2 \<cdot> s$2 \<cdot> s$0 - 2 \<cdot> s$2 \<cdot> h - s$1 \<cdot> s$1 = 0" in dCut)
+    apply(rule_tac I="\<lambda> s. 2 \<cdot> s$2 \<cdot> s$0 - 2 \<cdot> s$2 \<cdot> h - s$1 \<cdot> s$1 = 0" in dI)
+  using energy_conservation_invariant apply(blast)
+     apply(force simp: p2r_def, force simp: p2r_def)
    apply(rule dWeakening, subst p2r_r2p_wp)
   apply(simp add: rel_antidomain_kleene_algebra.fbox_def)
   unfolding rel_antidomain_kleene_algebra.cond_def p2r_def
   by(auto simp: bb_real_arith rel_ad_def rel_antidomain_kleene_algebra.ads_d_def)
+
+no_notation constant_acceleration_kinematics_matrix ("A")
+
+no_notation constant_acceleration_kinematics_matrix_flow ("\<phi>\<^sub>A")
 
 end
